substitution/substitution_lemmas.v
@@ -1,156 +1,176 @@
-Add LoadPath "C:\Users\Ziga\Documents\Ziga_podatki\repositories\eeff-formalization\substitution".
-Add LoadPath "C:\Users\Ziga\Documents\Ziga_podatki\repositories\eeff-formalization\syntax".
-(* Add LoadPath "E:\Ziga_Podatki\faks\eeff-formalization\substitution". *)
-(* Add LoadPath "E:\Ziga_Podatki\faks\eeff-formalization\syntax". *)
+(* Add LoadPath "C:\Users\Ziga\Documents\Ziga_podatki\repositories\eeff-formalization\substitution". *)
+(* Add LoadPath "C:\Users\Ziga\Documents\Ziga_podatki\repositories\eeff-formalization\syntax". *)
+Add LoadPath "E:\Ziga_Podatki\faks\eeff-formalization\substitution".
+Add LoadPath "E:\Ziga_Podatki\faks\eeff-formalization\syntax".
 Require Export substitution syntax_lemmas.
-Require Import Le.
+Require Import Le Compare_dec Arith.
+Require Import Omega.
 
 (* ==================== Effects on getters ==================== *)
 
-Lemma shift_find_None h o i j :
-  find_case h o = None <-> find_case (h_shift h i j) o = None.
+Lemma shift_get_case_None h op i cut :
+  get_case h op = None <-> get_case (h_shift h i cut) op = None.
 Proof.
-constructor; intro; induction h; auto; simpl in *;
-destruct (o==o0) eqn:cmp; try discriminate; auto.
+constructor; intros; induction h; simpl in *; auto.
+all: destruct (op==o) eqn:cmp; try discriminate; auto.
 Qed.
 
 
-Lemma negshift_find_None h o i j :
-  find_case h o = None <-> find_case (h_negshift h i j) o = None.
+Lemma negshift_get_case_None h op i cut :
+  get_case h op = None <-> get_case (h_negshift h i cut) op = None.
 Proof.
-constructor; intro; induction h; auto; simpl in *;
-destruct (o==o0) eqn:cmp; try discriminate; auto.
+constructor; intro; induction h; simpl in *; auto.
+all: destruct (op==o) eqn:cmp; try discriminate; auto.
 Qed.
 
 
-Lemma sub_find_None h o i v_s :
-  find_case h o = None -> 
-  find_case (h_sub h (i, v_s)) o = None.
+Lemma sub_get_case_None h op i vs :
+  get_case h op = None <->  get_case (h_sub h (i, vs)) op = None.
 Proof.
-intro; induction h; simpl in *. auto.
-destruct (o==o0) eqn:cmp. discriminate. auto.
+constructor; intro; induction h; simpl in *; auto.
+all: destruct (op==o) eqn:cmp; try discriminate; auto.
 Qed.
 
 
-Lemma shift_find_Some h o i j c :
-  find_case h o = Some c -> 
-  find_case (h_shift h i j) o = Some (c_shift c i (2+j)).
+Lemma shift_get_case_Some h op i cut c :
+  get_case h op = Some c -> 
+  get_case (h_shift h i cut) op = Some (c_shift c i (2+cut)).
 Proof.
-intro; induction h; simpl in *. discriminate.
-destruct (o==o0) eqn:cmp. inv H. all: auto.
+intros gets; induction h; simpl in *. discriminate.
+destruct (op==o) eqn:cmp. inv gets. all: auto.
 Qed.
 
 
-Lemma negshift_find_Some h o i j c :
-  find_case h o = Some c -> 
-  find_case (h_negshift h i j) o = Some (c_negshift c i (2+j)).
+Lemma negshift_get_case_Some h op i cut c :
+  get_case h op = Some c -> 
+  get_case (h_negshift h i cut) op = Some (c_negshift c i (2+cut)).
 Proof.
-intro; induction h; simpl in *. discriminate.
-destruct (o==o0) eqn:cmp. inv H. all: auto.
+intros gets; induction h; simpl in *. discriminate.
+destruct (op==o) eqn:cmp. inv gets. all: auto.
 Qed.
 
 
-Lemma sub_find_Some h o i v_s c :
-  find_case h o = Some c -> 
-    find_case (h_sub h (i, v_s)) o 
-  = Some (c_sub c (2+i, v_shift v_s 2 0)).
+Lemma sub_get_case_Some h op i vs c :
+  get_case h op = Some c -> 
+  get_case (h_sub h (i, vs)) op = Some (c_sub c (2+i, v_shift vs 2 0)).
 Proof.
-intro; induction h; simpl in *. discriminate.
-destruct (o==o0) eqn:cmp. inv H. all: auto.
+intros gets; induction h; simpl in *. discriminate.
+destruct (op==o) eqn:cmp. inv gets. all: auto.
 Qed.
 
-(* ==================== Shift and Sub interactions ==================== *)
+(* ==================== Shift Arithmetic ==================== *)
 
-Lemma v_shift_0 cut v : v_shift v 0 cut = v
-with c_shift_0 cut c  : c_shift c 0 cut = c
-with h_shift_0 cut h  : h_shift h 0 cut = h.
+Fixpoint v_shift_0 cut v : v_shift v 0 cut = v
+with     c_shift_0 cut c : c_shift c 0 cut = c
+with     h_shift_0 cut h : h_shift h 0 cut = h.
 Proof.
 { revert cut. induction v; intros cut; simpl; try f_equal; auto.
-  destruct (cut <=? v); auto. }
+  destruct (cut <=? n); auto. }
 { revert cut. induction c; intros cut; simpl; f_equal; auto. }
 { revert cut. induction h; intros cut; simpl; f_equal; auto. }
 Qed.
 
-
 Lemma inst_shift_0 cut I : inst_shift I 0 cut = I.
 Proof.
-  intros. induction I; simpl; f_equal; auto. apply v_shift_0.
+induction I; simpl; f_equal; auto. apply v_shift_0.
 Qed.
 
-Lemma v_shift_shift n m cut v :
-  v_shift (v_shift v n cut) m cut = (v_shift v (n + m) cut)
-with c_shift_shift n m cut c :
-  c_shift (c_shift c n cut) m cut = (c_shift c (n + m) cut)
-with h_shift_shift n m cut h :
-  h_shift (h_shift h n cut) m cut = (h_shift h (n + m) cut).
+
+Fixpoint v_shift_shift n m cut v {struct v}:
+  v_shift (v_shift v n cut) m cut = (v_shift v (n+m) cut)
+with c_shift_shift n m cut c {struct c}:
+  c_shift (c_shift c n cut) m cut = (c_shift c (n+m) cut)
+with h_shift_shift n m cut h {struct h}:
+  h_shift (h_shift h n cut) m cut = (h_shift h (n+m) cut).
 Proof.
-{
-revert cut. induction v; intros cut; simpl; f_equal; auto.
-destruct (cut <=? v) eqn:cmp; simpl.
-- apply (leb_complete _ _) in cmp.
-  assert (cut <=? n + v = true) by (apply leb_correct; omega).
-  rewrite H. f_equal. omega.
-- rewrite cmp. reflexivity. }
+{ induction v; simpl; f_equal; auto.
+  destruct (cut<=?n0) eqn:cmp; simpl.
+  - apply (leb_complete _ _) in cmp.
+    assert (cut<=?n+n0=true) by (apply leb_correct; omega).
+    rewrite H. f_equal. omega.
+  - rewrite cmp. reflexivity. }
 { revert cut. induction c; intros cut; try destruct p; simpl; f_equal; auto. }
 { revert cut. induction h; intros cut; simpl; f_equal; auto. }
 Qed.
 
-Lemma inst_shift_shift n m cut (I:instantiation) :
+Lemma inst_shift_shift n m cut I :
   inst_shift (inst_shift I n cut) m cut = inst_shift I (n+m) cut.
 Proof.
-intros. induction I; simpl; f_equal; auto. apply v_shift_shift.
+induction I; simpl; f_equal; auto. apply v_shift_shift.
 Qed.
 
 
-Fixpoint v_shift_comm n i j d (v:val) {struct v}:
+Fixpoint v_negshift_shift n m cut v {struct v}:
+  (m <= n) ->
+  v_negshift (v_shift v n cut) m cut = (v_shift v (n - m) cut)
+
+with c_negshift_shift n m cut c {struct c}:
+  (m <= n) ->
+  c_negshift (c_shift c n cut) m cut = (c_shift c (n - m) cut)
+
+with h_negshift_shift n m cut h {struct h}:
+  (m <= n) ->  
+  h_negshift (h_shift h n cut) m cut = (h_shift h (n - m) cut).
+
+Proof.
+all: intros cmp.
+{ induction v; simpl; f_equal; auto.
+  destruct (cut<=?n0) eqn:cv; simpl.
+  - apply leb_complete in cv.
+    assert (cut<=?n+n0=true) by (apply leb_correct; omega).
+    rewrite H. f_equal. omega.
+  - rewrite cv. reflexivity. }
+{ induction c; simpl; f_equal; auto. }
+{ induction h; simpl; f_equal; auto. }
+Qed.
+
+(* ==================== Commutativity (Distributivity) ==================== *)
+
+Fixpoint v_shift_comm n i j d v {struct v}:
   i >= j ->
   v_shift (v_shift v n i) d j = v_shift (v_shift v d j) n (d+i)
 
-with c_shift_comm n i j d (c:comp) {struct c}:
+with c_shift_comm n i j d c {struct c}:
   i >= j ->
   c_shift (c_shift c n i) d j = c_shift (c_shift c d j) n (d+i)
 
-with h_shift_comm n i j d (h:hcases) {struct h}:
+with h_shift_comm n i j d h {struct h}:
   i >= j ->
   h_shift (h_shift h n i) d j = h_shift (h_shift h d j) n (d+i).
+
 Proof.
 {
 intros cmp. induction v; simpl.
 { clear v_shift_comm c_shift_comm h_shift_comm.
-  rename v into dbi.
-  destruct (i<=?dbi) eqn:cmpi; destruct (j<=?dbi) eqn:cmpj; simpl.
+  destruct (i<=?n0) eqn:cmpi; destruct (j<=?n0) eqn:cmpj; simpl.
   + apply leb_complete in cmpi. apply leb_complete in cmpj.
-    assert (j<=?n+dbi=true) by (apply leb_correct; omega).
-    assert (d+i<=?d+dbi=true) by (apply leb_correct; omega).
+    assert (j<=?n+n0=true) by (apply leb_correct; omega).
+    assert (d+i<=?d+n0=true) by (apply leb_correct; omega).
     rewrite H, H0. f_equal. omega.
   + apply leb_complete in cmpi. apply leb_complete_conv in cmpj. omega.
   + apply leb_complete_conv in cmpi. rewrite cmpj. apply leb_complete in cmpj.
-    assert (d+i<=?d+dbi=false) by (apply leb_correct_conv; omega).  
-    rewrite H. reflexivity.
+    assert (d+i<=?d+n0=false) by (apply leb_correct_conv; omega).  
+    rewrite H. auto.
   + rewrite cmpj. 
     apply leb_complete_conv in cmpi. apply leb_complete_conv in cmpj.
-    assert (d+i<=?dbi=false) by (apply leb_correct_conv; omega).
-    rewrite H.  reflexivity.
-}
-clear v_shift_comm h_shift_comm.
+    assert (d+i<=?n0=false) by (apply leb_correct_conv; omega).
+    rewrite H. auto. }
 all: f_equal; auto.
-all: assert (S(d+i)=d+S i) by omega; rewrite H. 
+all: assert (S(d+i)=d+S i) as same by omega; rewrite same. 
 all: eapply c_shift_comm; omega.
 }{
-intros cmp. induction c; simpl; f_equal; auto; 
-clear v_shift_comm h_shift_comm.
-all: assert (S(S(d+i))=d+S(S i)) by omega; 
-  try (rewrite H; eapply c_shift_comm; omega).
-all: assert (S(d+i)=d+S i) by omega; rewrite H0; eapply c_shift_comm; omega.
+intros cmp. induction c; simpl; f_equal; eauto. 
+all: assert (S(S(d+i))=d+S(S i)) as ssame by omega.
+all: assert (S(d+i)=d+S i) as same by omega.
+all: try rewrite ssame; try rewrite same; eapply c_shift_comm; omega.
 }{
-clear v_shift_comm h_shift_comm.
-intros cmp. induction h; simpl.
-all: f_equal; auto.
-assert (S(S(d+i))=d+S(S i)) by omega; rewrite H; eapply c_shift_comm; omega.
+intros cmp. induction h; simpl; f_equal; auto.
+assert (S(S(d+i))=d+S(S i)) as ssame by omega. rewrite ssame.
+eapply c_shift_comm; omega.
 }
 Qed.
 
-Lemma inst_shift_comm n i j d (I:instantiation) :
+Lemma inst_shift_comm n i j d I:
   i>=j ->
   inst_shift (inst_shift I n i) d j = inst_shift (inst_shift I d j) n (d+i).
 Proof.
@@ -158,154 +178,106 @@ intros. induction I; simpl; f_equal; auto. apply v_shift_comm. omega.
 Qed.
 
 
-Lemma v_negshift_shift n m cut (v:val) :
-  (m <= n) ->
-  v_negshift (v_shift v n cut) m cut = (v_shift v (n - m) cut)
-
-with c_negshift_shift n m cut (c:comp) :
-  (m <= n) ->
-  c_negshift (c_shift c n cut) m cut = (c_shift c (n - m) cut)
-
-with h_negshift_shift n m cut (h:hcases) :
-  (m <= n) ->  
-  h_negshift (h_shift h n cut) m cut = (h_shift h (n - m) cut).
-Proof.
-{
-clear v_negshift_shift.
-revert cut. induction v; intros cut m_le_n; simpl; f_equal; auto.
-rename v into i. simpl. destruct (cut <=? i) eqn:cmp; simpl.
-- apply leb_complete in cmp.
-  assert (cut <=? n + i=true) by (apply leb_correct; omega).
-  rewrite H. f_equal. omega.
-- rewrite cmp. reflexivity.
-}{
-clear c_negshift_shift h_negshift_shift.
-revert cut. induction c; intros cut m_le_n; simpl; f_equal;
-try apply v_negshift_shift || apply IHc || apply IHc1 || apply IHc2; assumption.
-}{
-clear h_negshift_shift v_negshift_shift.
-revert cut. induction h; intros cut m_le_n; simpl; f_equal.
-reflexivity. apply IHh. assumption. apply c_negshift_shift. assumption.
-}
-Qed.
-
-
-Lemma v_shift_negshift_comm v n i j :
+Fixpoint v_shift_negshift_comm v n i j {struct v}:
   v_no_var v j -> i <= j ->
-    v_shift (v_negshift v 1 j) n i 
-  = v_negshift (v_shift v n i) 1 (n+j)
+  v_shift (v_negshift v 1 j) n i = v_negshift (v_shift v n i) 1 (n+j)
 
-with c_shift_negshift_comm c n i j :
+with c_shift_negshift_comm c n i j {struct c}:
   c_no_var c j -> i <= j ->
-    c_shift (c_negshift c 1 j) n i 
-  = c_negshift (c_shift c n i) 1 (n+j)
+  c_shift (c_negshift c 1 j) n i = c_negshift (c_shift c n i) 1 (n+j)
 
-with h_shift_negshift_comm h n i j :
+with h_shift_negshift_comm h n i j {struct h}:
   h_no_var h j -> i <= j ->
-    h_shift (h_negshift h 1 j) n i 
-  = h_negshift (h_shift h n i) 1 (n+j).
+  h_shift (h_negshift h 1 j) n i = h_negshift (h_shift h n i) 1 (n+j).
+
 Proof.
+all: intros novar cmp.
 {
-clear v_shift_negshift_comm.
-revert j; induction v; intros j novar cmpij; simpl.
-{ 
-rename v into d. simpl. destruct (j<=?d) eqn:jd.
-+ apply leb_complete in jd. 
-  assert (i<=?d=true) by (apply leb_correct; omega).
-  rewrite H. simpl. assert (n+j<=?n+d=true) by (apply leb_correct; omega).
-  rewrite H0. assert (i<=?d-1=true).
-  { apply leb_correct. simpl in novar. omega. }
-  rewrite H1. f_equal. simpl in novar. omega.
-+ apply leb_complete_conv in jd. simpl.
-  destruct (i<=?d) eqn:id; simpl.
-  - assert (n+j<=?n+d=false) by (apply leb_correct_conv; omega).
-    rewrite H. reflexivity.
-  - assert (n+j<=?d=false) by (apply leb_correct_conv; omega).
-    rewrite H. reflexivity.
-}
-all : f_equal; simpl in novar; try destruct novar; auto.
-all : assert (S(n+j)=n+(S j)) as snj by omega; rewrite snj.
-all : apply c_shift_negshift_comm; omega || auto.
+destruct v; simpl in *; auto.
+{ destruct (j<=?n0) eqn:jn0.
+  + apply leb_complete in jn0. 
+    assert (i<=?n0=true) by (apply leb_correct; omega). rewrite H. simpl.
+    assert (n+j<=?n+n0=true) by (apply leb_correct; omega). rewrite H0.
+    assert (i<=?n0-1=true) by (apply leb_correct; omega). rewrite H1.
+    f_equal. aomega.
+  + apply leb_complete_conv in jn0. simpl.
+    destruct (i<=?n0) eqn:in0; simpl.
+    - assert (n+j<=?n+n0=false) by (apply leb_correct_conv; omega).
+      rewrite H. auto.
+    - assert (n+j<=?n0=false) by (apply leb_correct_conv; omega).
+      rewrite H. auto. }
+all: f_equal; simpl in novar; try destruct novar; auto.
+all: assert (S(n+j)=n+(S j)) as same by omega; rewrite same.
+all: apply c_shift_negshift_comm; aomega.
 }{
-clear h_shift_negshift_comm.
-revert j. destruct c; intros j novar cmpij; simpl in *; f_equal; auto.
-all : assert (S(S(n+j))=n+(S (S j))) as ssnj by omega; try rewrite ssnj.
-all : assert (S(n+j)=n+(S j)) as snj by omega; try rewrite snj.
-all: apply v_shift_negshift_comm || apply c_shift_negshift_comm.
-all: omega || (try destruct novar; auto).
-all: destruct H0; auto.
+destruct c; simpl in *; f_equal; auto.
+all: assert (S(S(n+j))=n+(S (S j))) as ssame by omega; try rewrite ssame.
+all: assert (S(n+j)=n+(S j)) as same by omega; try rewrite same.
+all: try destruct novar; try destruct H0; auto.
+all: apply c_shift_negshift_comm; aomega.
 }{
-clear h_shift_negshift_comm v_shift_negshift_comm.
-revert j. induction h; intros j novar cmpij; simpl; f_equal. auto.
-+ inv novar; auto.
-+ assert (S(S(n+j))=n+(S (S j))) as ssnj by omega; try rewrite ssnj.
-  apply c_shift_negshift_comm. inv novar. auto. omega.
+destruct h; simpl in *; f_equal; try destruct novar; auto.
+assert (S(S(n+j))=n+(S(S j))) as ssame by omega; try rewrite ssame.
+apply c_shift_negshift_comm; aomega.
 }
 Qed.
 
 Lemma inst_shift_negshift_comm I n i j :
   inst_no_var I j -> i <= j ->
-    inst_shift (inst_negshift I 1 j) n i 
+    inst_shift (inst_negshift I 1 j) n i
   = inst_negshift (inst_shift I n i) 1 (n+j).
 Proof.
-revert n i j. induction I; intros; simpl; f_equal. auto.
-all: simpl in H; destruct H. auto.
-apply v_shift_negshift_comm. auto. omega.
+revert n i j. induction I; intros n i j novar cmp; simpl; f_equal. auto.
+all: simpl in novar; destruct novar. auto.
+apply v_shift_negshift_comm; aomega.
 Qed.
 
 
-Lemma v_shift_negshift_comm_alt v i j :
+Lemma v_shift_negshift_comm_alt v i j:
   v_no_var v j -> j < i ->
-    v_shift (v_negshift v 1 j) 1 i 
-  = v_negshift (v_shift v 1 (1+i)) 1 j
+  v_shift (v_negshift v 1 j) 1 i = v_negshift (v_shift v 1 (1+i)) 1 j
 
-with c_shift_negshift_comm_alt c i j :
+with c_shift_negshift_comm_alt c i j:
   c_no_var c j -> j < i ->
-    c_shift (c_negshift c 1 j) 1 i 
-  = c_negshift (c_shift c 1 (1+i)) 1 j
+  c_shift (c_negshift c 1 j) 1 i = c_negshift (c_shift c 1 (1+i)) 1 j
 
-with h_shift_negshift_comm_alt h i j :
+with h_shift_negshift_comm_alt h i j:
   h_no_var h j -> j < i ->
-    h_shift (h_negshift h 1 j) 1 i 
-  = h_negshift (h_shift h 1 (1+i)) 1 j.
+  h_shift (h_negshift h 1 j) 1 i = h_negshift (h_shift h 1 (1+i)) 1 j.
+
 Proof.
+all: intros novar cmp.
 {
-clear v_shift_negshift_comm_alt.
-revert j; induction v; intros j novar cmpij.
-{ 
-assert (1+i=i+1) as hack by omega. rewrite hack.
-rename v into d. simpl. destruct (j<=?d) eqn:jd.
-+ apply leb_complete in jd. simpl in novar.
-  destruct (i+1<=?d) eqn:sid; simpl.
-  - assert (j<=? S d=true) by (apply leb_correct; omega).
-    rewrite H. destruct d; simpl. omega. apply leb_complete in sid.
-    assert (i<=?d-0=true) by (apply leb_correct; omega).
-    rewrite H0. f_equal. omega.
-  - apply leb_complete_conv in sid. apply leb_correct in jd as jd'.
-    rewrite jd'. destruct d. omega. 
-    assert (i<=?S d-1=false) by (apply leb_correct_conv; omega). 
-    rewrite H. reflexivity.
-+ simpl. apply leb_complete_conv in jd as jd'. 
-  assert (i<=?d=false) by (apply leb_correct_conv; omega). rewrite H.
-  assert (i+1<=?d=false) by (apply leb_correct_conv; omega). rewrite H0.
-  simpl. rewrite jd. reflexivity.
-}
-all : simpl; auto; f_equal; simpl in novar; try destruct novar; auto.
-all : apply c_shift_negshift_comm_alt; omega || auto.
+destruct v.
+{ assert (1+i=i+1) as hack by omega. rewrite hack. clear hack.
+  rename n into d. simpl. destruct (j<=?d) eqn:jd.
+  + apply leb_complete in jd. simpl in novar.
+    destruct (i+1<=?d) eqn:sid; simpl.
+    - assert (j<=? S d=true) by (apply leb_correct; omega).
+      rewrite H. destruct d; simpl. omega. apply leb_complete in sid.
+      assert (i<=?d-0=true) by (apply leb_correct; omega).
+      rewrite H0. f_equal. omega.
+    - apply leb_complete_conv in sid. apply leb_correct in jd as jd'.
+      rewrite jd'. destruct d. omega.
+      assert (i<=?S d-1=false) by (apply leb_correct_conv; omega). 
+      rewrite H. auto.
+  + simpl. apply leb_complete_conv in jd as jd'. 
+    assert (i<=?d=false) by (apply leb_correct_conv; omega). rewrite H.
+    assert (i+1<=?d=false) by (apply leb_correct_conv; omega). rewrite H0.
+    simpl. rewrite jd. auto. }
+all: simpl in *; auto; f_equal; try destruct novar; auto.
+all: apply c_shift_negshift_comm_alt; aomega.
 }{
-clear h_shift_negshift_comm_alt.
-revert j. destruct c; intros j novar cmpij; simpl in *; f_equal; auto.
-all: apply v_shift_negshift_comm_alt || apply c_shift_negshift_comm_alt; auto.
-all: omega || (try destruct novar; auto).
-all: destruct H0; auto.
+destruct c; simpl in *; f_equal; auto.
+all: try destruct novar; try destruct H0; auto.
+all: apply c_shift_negshift_comm_alt; aomega.
 }{
-clear v_shift_negshift_comm_alt. 
-revert j. induction h; intros j novar cmpij; simpl in *; f_equal. auto.
-all: destruct novar; auto. apply c_shift_negshift_comm_alt. auto. omega.
+destruct h; simpl in *; f_equal; auto.
+all: try destruct novar; auto. apply c_shift_negshift_comm_alt; aomega.
 }
 Qed.
 
-(* ==================== novar interactions ==================== *)
+(* ==================== NoVar Interactions ==================== *)
 
 Lemma v_shift_makes_no_var v j:
   v_no_var (v_shift v 1 j) j
@@ -314,147 +286,147 @@ with c_shift_makes_no_var c j:
 with h_shift_makes_no_var h j:
   h_no_var (h_shift h 1 j) j.
 Proof.
-{clear v_shift_makes_no_var.
-revert j; induction v; intros j; simpl; auto.
-destruct (j<=?v) eqn:cmp; simpl.
-+ apply leb_complete in cmp. omega.
-+ apply leb_iff_conv in cmp. omega. }
-{revert j; induction c; intros j; try destruct p; simpl; auto. }
-{revert j; induction h; intros j; simpl; auto. }
+{ revert j; induction v; intros j; simpl; auto.
+  destruct (j<=?n) eqn:cmp; simpl.
+  + apply leb_complete in cmp. omega.
+  + apply leb_iff_conv in cmp. omega. }
+{ revert j; induction c; intros j; try destruct p; simpl; auto. }
+{ revert j; induction h; intros j; simpl; auto. }
 Qed.
 
 
-Lemma v_no_var_shift (v:val) j n cut:
-  v_no_var v j -> (cut <= j) -> v_no_var (v_shift v n cut) (n+j)
-with c_no_var_shift (c:comp) j n cut:
-  c_no_var c j -> (cut <= j) -> c_no_var (c_shift c n cut) (n+j)
-with h_no_var_shift (h:hcases) j n cut:
-  h_no_var h j -> (cut <= j) -> h_no_var (h_shift h n cut) (n+j).
+Fixpoint v_no_var_shift v j n cut:
+  v_no_var v j -> (cut <= j) -> 
+  v_no_var (v_shift v n cut) (n+j)
+
+with c_no_var_shift c j n cut:
+  c_no_var c j -> (cut <= j) -> 
+  c_no_var (c_shift c n cut) (n+j)
+
+with h_no_var_shift h j n cut:
+  h_no_var h j -> (cut <= j) -> 
+  h_no_var (h_shift h n cut) (n+j).
+
 Proof.
 all: assert (forall j, S(n+j)=n+(S j)) as snj by (intro; omega).
 all: assert (forall j, S(S(n+j))=n+(S(S j))) as ssnj by (intro; omega).
+all: intros orig cmp.
 {
-clear v_no_var_shift.
-revert j. induction v; intros j orig cmpjc; simpl; simpl in orig;
-try constructor; try inv orig; auto.
-{ destruct (cut <=? v) eqn:cmp; simpl; try rewrite leb_iff_conv in cmp; omega. }
-all: rewrite snj; apply c_no_var_shift; omega || assumption.
+destruct v; simpl in *.
+{ destruct (cut <=? n0) eqn:cn; simpl; try rewrite leb_iff_conv in cn; omega. }
+all: try constructor; try destruct orig; auto.
+all: rewrite snj; apply c_no_var_shift; aomega.
 }{
-clear c_no_var_shift.
-revert j cut. induction c; intros j cut orig cmpjc; simpl; simpl in *.
-all: try inv orig; try constructor; try constructor; auto.
-all: try rewrite ssnj; try rewrite snj.
-all: try apply IHc || apply IHc1 || apply IHc2; omega || auto.
-all: inv H0; assumption.
+destruct c; simpl in *; auto.
+all: try destruct orig; try destruct H0; try constructor; try constructor; auto.
+all: try rewrite ssnj; try rewrite snj; apply c_no_var_shift; aomega.
 }{
-clear h_no_var_shift.
-revert j cut. induction h; intros j cut orig cmpjc; simpl;
-destruct orig; auto. constructor. auto.
-rewrite ssnj. apply c_no_var_shift. assumption. omega.
+destruct h; simpl in *; auto.
+destruct orig. constructor; auto. rewrite ssnj. apply c_no_var_shift; aomega.
 }
 Qed.
 
 
-Lemma inst_no_var_shift I j n cut:
-  inst_no_var I j -> (cut <= j) -> inst_no_var (inst_shift I n cut) (n+j).
+Fixpoint inst_no_var_shift I j n cut {struct I}:
+  inst_no_var I j -> (cut <= j) -> 
+  inst_no_var (inst_shift I n cut) (n+j).
 Proof.
-revert j n cut. induction I; intros; simpl; auto.
-simpl in H. destruct H. constructor; eauto.
-apply v_no_var_shift. auto. omega.
+intros orig cmp. destruct I; simpl in *; auto.
+destruct orig. constructor; eauto. apply v_no_var_shift; aomega.
 Qed.
 
 
-Lemma v_no_var_shift_alt (v:val) j n cut:
-  v_no_var v j -> (cut > j) -> v_no_var (v_shift v n cut) j
-with c_no_var_shift_alt (c:comp) j n cut:
-  c_no_var c j -> (cut > j) -> c_no_var (c_shift c n cut) j
-with h_no_var_shift_alt (h:hcases) j n cut:
-  h_no_var h j -> (cut > j) -> h_no_var (h_shift h n cut) j.
+Fixpoint v_no_var_shift_alt v j n cut:
+  v_no_var v j -> (cut > j) ->
+  v_no_var (v_shift v n cut) j
+
+with c_no_var_shift_alt c j n cut:
+  c_no_var c j -> (cut > j) ->
+  c_no_var (c_shift c n cut) j
+
+with h_no_var_shift_alt h j n cut:
+  h_no_var h j -> (cut > j) ->
+  h_no_var (h_shift h n cut) j.
+
 Proof.
+all: intros orig cmp.
 {
-clear v_no_var_shift_alt.
-revert j. induction v; intros j orig cmpjc; simpl; simpl in orig;
-try constructor; try inv orig; auto.
-{ destruct (cut <=? v) eqn:cmp; simpl; omega || auto.
-  rewrite leb_iff in cmp; omega. }
-all: apply c_no_var_shift_alt; omega || assumption.
+destruct v; simpl in *.
+{ destruct (cut <=? n0) eqn:cn; simpl; try apply leb_complete in cn; omega. }
+all: try constructor; try destruct orig; auto.
+all: apply c_no_var_shift_alt; aomega.
 }{
-clear c_no_var_shift_alt.
-revert j cut. induction c; intros j cut orig cmpjc; simpl; simpl in *.
-all: try inv orig; try constructor; try constructor; auto.
-all: try apply IHc || apply IHc1 || apply IHc2; omega || auto.
-all: inv H0; assumption.
+destruct c; simpl in *; auto.
+all: try destruct orig; try destruct H0; try constructor; try constructor; auto.
+all: apply c_no_var_shift_alt; aomega.
 }{
-clear h_no_var_shift_alt.
-revert j cut. induction h; intros j cut orig cmpjc; simpl;
-destruct orig; auto. constructor. auto. apply c_no_var_shift_alt; omega || auto.
+destruct h; simpl in *; auto.
+destruct orig. constructor; auto. apply c_no_var_shift_alt; aomega.
 }
 Qed.
 
 
-Lemma v_sub_makes_no_var (v:val) j v_s :
-  v_no_var v_s j -> v_no_var (v_sub v (j, v_s)) j
-with c_sub_makes_no_var (c:comp) j v_s :
-  v_no_var v_s j -> c_no_var (c_sub c (j, v_s)) j
-with h_sub_makes_no_var (h:hcases) j v_s :
-  v_no_var v_s j -> h_no_var (h_sub h (j, v_s)) j.
+Fixpoint v_sub_makes_no_var v j vs :
+  v_no_var vs j -> v_no_var (v_sub v (j, vs)) j
+with c_sub_makes_no_var c j vs :
+  v_no_var vs j -> c_no_var (c_sub c (j, vs)) j
+with h_sub_makes_no_var h j vs :
+  v_no_var vs j -> h_no_var (h_sub h (j, vs)) j.
 Proof.
+all: intros novar.
 {
-clear v_sub_makes_no_var.
-revert j. induction v; intros j v_s_clean; try constructor.
-all: try (apply IHv; assumption); auto.
-{simpl. destruct (v =? j) eqn:vj; auto. simpl. apply Nat.eqb_neq in vj. omega. }
-all: apply c_sub_makes_no_var; apply v_no_var_shift; omega || assumption.
+destruct v; simpl in *; auto.
+{ destruct (n=?j) eqn:nj; auto. simpl. apply Nat.eqb_neq in nj. omega. }
+all: try aconstructor; apply c_sub_makes_no_var; apply v_no_var_shift; aomega.
 }{
-clear c_sub_makes_no_var.
-revert j v_s. induction c; intros j v_s v_s_clean; simpl.
+destruct c; simpl in *; auto.
 all: try constructor; try constructor; auto.
-all: try apply IHc || apply IHc1 || apply IHc2; auto.
 all: assert (S(S j)=2+j) as ssj by omega; try rewrite ssj.
-all: try apply v_no_var_shift; omega || auto.
+all: apply c_sub_makes_no_var; apply v_no_var_shift; aomega.
 }{
-clear h_sub_makes_no_var.
-revert j v_s. induction h; intros j v_s v_s_clean; simpl; auto.
-constructor. auto. assert (S(S j)=2+j) as ssj by omega. rewrite ssj.
-apply c_sub_makes_no_var. apply v_no_var_shift. assumption. omega.
+destruct h; simpl in *; try constructor; auto.
+assert (S(S j)=2+j) as ssj by omega. rewrite ssj.
+apply c_sub_makes_no_var; apply v_no_var_shift; aomega.
 }
 Qed.
-
 
 Lemma inst_sub_makes_no_var I j v_s :
   v_no_var v_s j -> inst_no_var (inst_sub I (j, v_s)) j.
 Proof.
-revert j. induction I; intros; simpl. auto. constructor.
-+ apply v_sub_makes_no_var. auto.
-+ auto.
+revert j. induction I; intros; simpl. auto. aconstructor.
+apply v_sub_makes_no_var. auto.
 Qed.
 
 
 Fixpoint v_under_var_shift v j n cut:
-  v_under_var v j -> cut <= j -> v_under_var (v_shift v n cut) (n+j)
+  v_under_var v j -> cut <= j -> 
+  v_under_var (v_shift v n cut) (n+j)
+
 with c_under_var_shift c j n cut:
-  c_under_var c j -> cut <= j -> c_under_var (c_shift c n cut) (n+j)
+  c_under_var c j -> cut <= j -> 
+  c_under_var (c_shift c n cut) (n+j)
+
 with h_under_var_shift h j n cut:
-  h_under_var h j -> cut <= j -> h_under_var (h_shift h n cut) (n+j).
+  h_under_var h j -> cut <= j -> 
+  h_under_var (h_shift h n cut) (n+j).
+
 Proof.
-all: assert (S(n+j)=n+S j) as Snj by omega.
-all: assert (S(S(n+j))=n+S(S j)) as SSnj by omega.
+all: assert (S(n+j)=n+S j) as snj by omega.
+all: assert (S(S(n+j))=n+S(S j)) as ssnj by omega.
+all: intros under cmp. 
 {
-intros under cmp. destruct v; simpl; simpl in under; auto.
-{ destruct (cut <=? v) eqn:ccmp; simpl; omega. }
-all: try (destruct under; constructor; auto).
-all: rewrite Snj; eapply c_under_var_shift; eauto; omega.
+destruct v; simpl in *; auto.
+{ destruct (cut <=? n0) eqn:ccmp; simpl; omega. }
+all: try constructor; try destruct under; auto.
+all: rewrite snj; eapply c_under_var_shift; aomega.
 }{
-intros under cmp. destruct c; simpl; simpl in under; auto.
-all: try (destruct under; constructor; auto).
-all: try rewrite SSnj; try rewrite Snj.
-2: destruct H0; constructor.
-4: destruct H0; constructor.
-all: eapply c_under_var_shift; eauto; omega.
+destruct c; simpl in *; auto.
+all: try destruct under; try destruct H0; try constructor; try constructor.
+all: try rewrite ssnj; try rewrite snj; auto.
+all: eapply c_under_var_shift; aomega.
 }{
-intros under cmp. destruct h; simpl; simpl in under. auto.
-destruct under. constructor. auto.
-rewrite SSnj. eapply c_under_var_shift; eauto; omega.
+destruct h; simpl in *. auto. destruct under. constructor. auto.
+rewrite ssnj. eapply c_under_var_shift; aomega.
 }
 Qed.
 
@@ -467,16 +439,15 @@ with h_shift_too_high h n cut :
   h_under_var h cut -> h_shift h n cut = h.
 Proof.
 {
-intros under. destruct v; simpl; simpl in under.
-{ assert (cut <=? v = false) by (apply leb_correct_conv; omega).
-  rewrite H. reflexivity. }
-all: try (destruct under; f_equal; auto) || (f_equal; auto).
+intros under. destruct v; simpl in *.
+{ assert (cut<=?n0=false) by (apply leb_correct_conv; omega). rewrite H. auto. }
+all: try destruct under; f_equal; auto.
 }{
-intros under. destruct c; simpl; simpl in under.
-all: try (destruct under; f_equal; auto) || (f_equal; auto); destruct H0; auto.
+intros under. destruct c; simpl in *.
+all: try destruct under; try destruct H0; f_equal; auto.
 }{
-intros under. destruct h; simpl; simpl in under.
-all: try (destruct under; f_equal; auto) || (f_equal; auto).
+intros under. destruct h; simpl in *.
+all: try destruct under; f_equal; auto.
 }
 Qed.
 
@@ -489,16 +460,15 @@ with h_negshift_too_high h n cut :
   h_under_var h cut -> h_negshift h n cut = h.
 Proof.
 {
-intros under. destruct v; simpl; simpl in under.
-{ assert (cut <=? v = false) by (apply leb_correct_conv; omega).
-  rewrite H. reflexivity. }
-all: try (destruct under; f_equal; auto) || (f_equal; auto).
+intros under. destruct v; simpl in *.
+{ assert (cut<=?n0=false) by (apply leb_correct_conv; omega). rewrite H. auto. }
+all: try destruct under; f_equal; auto.
 }{
-intros under. destruct c; simpl; simpl in under.
-all: try (destruct under; f_equal; auto) || (f_equal; auto); destruct H0; auto.
+intros under. destruct c; simpl in *.
+all: try destruct under; try destruct H0; f_equal; auto.
 }{
-intros under. destruct h; simpl; simpl in under.
-all: try (destruct under; f_equal; auto) || (f_equal; auto).
+intros under. destruct h; simpl in *.
+all: try destruct under; f_equal; auto.
 }
 Qed.
 
@@ -511,120 +481,111 @@ with h_sub_too_high h i v_s:
   h_under_var h i -> h_sub h (i, v_s) = h.
 Proof.
 {
-intros under. destruct v; simpl; simpl in under.
-{ assert (v=?i=false) by (apply Nat.eqb_neq; omega).
-  rewrite H. reflexivity. }
-all: try (destruct under; f_equal; auto) || (f_equal; auto).
+intros under. destruct v; simpl in *.
+{ assert (n=?i=false) by (apply Nat.eqb_neq; omega). rewrite H. auto. }
+all: try destruct under; f_equal; auto.
 }{
-intros under. destruct c; simpl; simpl in under.
-all: try (destruct under; f_equal; auto) || (f_equal; auto); destruct H0; auto.
+intros under. destruct c; simpl in *.
+all: try destruct under; try destruct H0; f_equal; auto.
 }{
-intros under. destruct h; simpl; simpl in under.
-all: try (destruct under; f_equal; auto) || (f_equal; auto).
+intros under. destruct h; simpl in *.
+all: try destruct under; f_equal; auto.
 }
 Qed.
+
 
 Fixpoint v_subs_too_high v i v_s:
-v_under_var v i -> v_subs v i v_s = v
+  v_under_var v i -> v_subs v i v_s = v
 with c_subs_too_high c i v_s:
-c_under_var c i -> c_subs c i v_s = c
+  c_under_var c i -> c_subs c i v_s = c
 with h_subs_too_high h i v_s:
-h_under_var h i -> h_subs h i v_s = h.
+  h_under_var h i -> h_subs h i v_s = h.
 Proof.
 {
-intros under. unfold v_subs. 
-rewrite v_sub_too_high, v_negshift_too_high; auto.
+intros under. unfold v_subs. rewrite v_sub_too_high, v_negshift_too_high; auto.
 }{
-intros under. unfold c_subs. 
-rewrite c_sub_too_high, c_negshift_too_high; auto.
+intros under. unfold c_subs. rewrite c_sub_too_high, c_negshift_too_high; auto.
 }{
-intros under. unfold h_subs. 
-rewrite h_sub_too_high, h_negshift_too_high; auto.
+intros under. unfold h_subs. rewrite h_sub_too_high, h_negshift_too_high; auto.
 }
 Qed.
 
 
-
-Fixpoint v_sub_no_var v v' i {struct v}:
+Fixpoint v_sub_no_var_same v v' i {struct v}:
   v_no_var v i -> v_sub v (i, v') = v
-with c_sub_no_var c v' i {struct c}:
+with c_sub_no_var_same c v' i {struct c}:
   c_no_var c i -> c_sub c (i, v') = c
-with h_sub_no_var h v' i {struct h}:
+with h_sub_no_var_same h v' i {struct h}:
   h_no_var h i -> h_sub h (i, v') = h.
 Proof.
-all: revert i.
-+ intros i novar. destruct v; simpl in novar. 
-  { assert (v=?i=false) by (apply Nat.eqb_neq; omega).
-    simpl. rewrite H. reflexivity. }
-  all: try destruct novar; simpl in *; f_equal; auto.
-+ intros i novar. induction c; simpl in *; try destruct novar.
-  all: f_equal; auto. all: destruct H0; auto.
-+ intros i novar. induction h; simpl in *; try destruct novar.
-  all: f_equal; auto.
+all: intros novar.
++ destruct v; simpl in *. 
+  { assert (n=?i=false) by (apply Nat.eqb_neq; omega). rewrite H. auto. }
+  all: try destruct novar; f_equal; auto.
++ induction c; simpl in *. 
+  all: try destruct novar; try destruct H0; f_equal; auto.
++ induction h; simpl in *; try destruct novar; f_equal; auto.
 Qed.
 
 (* ==================== Sub Interactions ==================== *)
 
-Lemma v_shift_sub v v' i cut j :
+Fixpoint v_shift_sub v v' i cut j {struct v}:
   cut <= j ->
     v_shift (v_sub v (j, v')) i cut 
   = v_sub (v_shift v i cut) (i+j, v_shift v' i cut)
 
-with c_shift_sub c v' i cut j :
+with c_shift_sub c v' i cut j {struct c}:
   cut <= j ->
     c_shift (c_sub c (j, v')) i cut 
   = c_sub (c_shift c i cut) (i+j, v_shift v' i cut)
 
-with h_shift_sub h v' i cut j :
+with h_shift_sub h v' i cut j {struct h}:
   cut <= j ->
     h_shift (h_sub h (j, v')) i cut
   = h_sub (h_shift h i cut) (i+j, v_shift v' i cut).
+
 Proof.
-all : assert (S(i+j)=i+(S j)) as sij by omega.
-all : assert (S(S(i+j))=i+(S (S j))) as ssij by omega.
-{
-revert cut; induction v; intros cut cmpcj; simpl.
-{ simpl. destruct (cut<=?v) eqn:cv.
-  + destruct (v=?j) eqn:vj.
-    * apply Nat.eqb_eq in vj. subst. simpl.
-      assert (i+j=?i+j=true) by (apply Nat.eqb_eq; omega).
-      rewrite H. reflexivity.
-    * simpl. rewrite cv. assert (i+v=?i+j=false).
-      { apply Nat.eqb_neq. apply Nat.eqb_neq in vj. omega. }
-      rewrite H. reflexivity.
-  + assert (v=?j=false).
-    { apply Nat.eqb_neq. apply leb_complete_conv in cv. omega. }
-    rewrite H. simpl. rewrite cv.
-    assert (v=?i+j=false).
-    { apply Nat.eqb_neq. apply leb_complete_conv in cv. omega. }
-    rewrite H0. reflexivity.
-}
-all : f_equal; auto.
-all : rewrite sij, v_shift_comm, c_shift_sub; try omega || f_equal.
+all: assert (S(i+j)=i+(S j)) as Sij by omega.
+all: assert (S(S(i+j))=i+(S(S j))) as SSij by omega.
+all: intros cmp.
+{ destruct v; simpl in *.
+  { simpl. destruct (cut<=?n) eqn:cn.
+    + destruct (n=?j) eqn:nj.
+      * apply Nat.eqb_eq in nj. subst. simpl.
+        assert (i+j=?i+j=true) by (apply Nat.eqb_eq; omega).
+        rewrite H. auto.
+      * simpl. rewrite cn. assert (i+n=?i+j=false).
+        { apply Nat.eqb_neq. apply Nat.eqb_neq in nj. omega. }
+        rewrite H. auto.
+    + assert (n=?j=false).
+      { apply Nat.eqb_neq. apply leb_complete_conv in cn. omega. }
+      rewrite H. simpl. rewrite cn.
+      assert (n=?i+j=false).
+      { apply Nat.eqb_neq. apply leb_complete_conv in cn. omega. }
+      rewrite H0. auto. }
+all: f_equal; auto.
+all: rewrite Sij, v_shift_comm, c_shift_sub; aomega.
 }{
-clear h_shift_sub.
-revert cut; induction c; intros cut cmpcj; simpl; f_equal; auto.
-all : try rewrite ssij; try rewrite sij.
-all: rewrite v_shift_comm, c_shift_sub; try omega || f_equal.
+destruct c; simpl in *; f_equal; auto.
+all : try rewrite SSij; try rewrite Sij.
+all: rewrite v_shift_comm, c_shift_sub; aomega.
 }{
-clear v_shift_sub h_shift_sub.
-revert cut; induction h; intros cut cmpcj; simpl; f_equal; auto.
-+ rewrite ssij, v_shift_comm, c_shift_sub; try omega || f_equal.
+destruct h; simpl in *; f_equal; auto.
+rewrite SSij, v_shift_comm, c_shift_sub; aomega.
 }
 Qed.
 
-
-Lemma inst_shift_sub I v' i cut j :
+Fixpoint inst_shift_sub I v' i cut j {struct I}:
   cut <= j ->
     inst_shift (inst_sub I (j, v')) i cut 
   = inst_sub (inst_shift I i cut) (i+j, v_shift v' i cut).
 Proof.
-revert i cut j. induction I; intros; simpl; f_equal; auto.
+destruct I; intros; simpl; f_equal; auto.
 apply v_shift_sub. omega.
 Qed.
 
 
-Lemma v_negshift_sub v v' cut j :
+Fixpoint v_negshift_sub v v' cut j :
   cut < j -> v_no_var v cut -> v_no_var v' cut ->
     v_negshift (v_sub v (j, v')) 1 cut 
   = v_sub (v_negshift v 1 cut) (j-1, v_negshift v' 1 cut)
@@ -638,88 +599,75 @@ with h_negshift_sub h v' cut j :
   cut < j -> h_no_var h cut -> v_no_var v' cut ->
     h_negshift (h_sub h (j, v')) 1 cut
   = h_sub (h_negshift h 1 cut) (j-1, v_negshift v' 1 cut).
+
 Proof.
+all: intros cmp novar novar'.
 {
-revert cut j; induction v; intros cut j cmpcj novar novar'; simpl.
-{ 
-rename v into d. simpl. simpl in novar.
-destruct (cut<=?d) eqn:cd.
-+ destruct (d=?j) eqn:dsj.
-  - simpl. apply Nat.eqb_eq in dsj. subst.
-    assert (j-1=?j-1=true) by (apply Nat.eqb_eq; omega).
-    rewrite H. reflexivity.
-  - simpl. rewrite cd. assert (d-1=?j-1=false).
-    { apply Nat.eqb_neq. apply Nat.eqb_neq in dsj. omega. }
-    rewrite H. reflexivity.
-+ assert (d=?j=false).
-  { apply Nat.eqb_neq. apply leb_complete_conv in cd. omega. }
-  rewrite H. simpl. rewrite cd.
-  assert (d=?j-1=false).
-  { apply Nat.eqb_neq. apply leb_complete_conv in cd. omega. }
-  rewrite H0. reflexivity.
-}
-all : simpl in novar; try (destruct novar; auto); f_equal; auto.
-all : rewrite c_negshift_sub; try omega || (f_equal; f_equal; omega || auto).
-all : clear v_negshift_sub c_negshift_sub h_negshift_sub.
-all : try rewrite v_shift_negshift_comm; f_equal || omega || auto.
-all : apply v_no_var_shift; omega || auto.
+destruct v; simpl in *.
+{ destruct (cut<=?n) eqn:cn.
+  + destruct (n=?j) eqn:nsj.
+    - simpl. apply Nat.eqb_eq in nsj. subst.
+      assert (j-1=?j-1=true) by (apply Nat.eqb_eq; omega).
+      rewrite H. auto.
+    - simpl. rewrite cn. assert (n-1=?j-1=false).
+      { apply Nat.eqb_neq. apply Nat.eqb_neq in nsj. omega. }
+      rewrite H. auto.
+  + assert (n=?j=false).
+    { apply Nat.eqb_neq. apply leb_complete_conv in cn. omega. }
+    rewrite H. simpl. rewrite cn.
+    assert (n=?j-1=false).
+    { apply Nat.eqb_neq. apply leb_complete_conv in cn. omega. }
+    rewrite H0. auto. }
+all: try destruct novar; f_equal; auto.
+all: rewrite c_negshift_sub; try do 2 f_equal; aomega.
+all: try rewrite v_shift_negshift_comm; aomega.
+all: apply v_no_var_shift; aomega.
 }{
-clear h_negshift_sub.
-revert cut j; induction c; intros cut j cmpcj novar novar'; simpl.
-all : simpl in novar; try destruct novar; f_equal; auto.
-all : clear v_negshift_sub.
-all : assert (S(S cut)=2+cut) as ssc by omega; try rewrite ssc.
-all : assert (S cut=1+cut) as sc by omega; try rewrite sc.
-all : try destruct H0.
-all : try rewrite c_negshift_sub; (f_equal; f_equal; try omega) || auto.
-all : try rewrite v_shift_negshift_comm; f_equal || omega || auto.
-all : try apply v_no_var_shift; omega || auto.
+destruct c; simpl in *.
+all: try destruct novar; try destruct H0; f_equal; auto.
+all: assert (S(S cut)=2+cut) as ssc by omega; try rewrite ssc.
+all: assert (S cut=1+cut) as sc by omega; try rewrite sc.
+all: rewrite c_negshift_sub; try do 2 f_equal; aomega.
+all: try rewrite v_shift_negshift_comm; aomega.
+all: try apply v_no_var_shift; aomega.
 }{
-clear v_negshift_sub h_negshift_sub.
-revert cut j; induction h; intros cut j cmpcj novar novar'.
-all : simpl; f_equal; simpl in novar; try destruct novar; auto.
-try rewrite c_negshift_sub. f_equal. f_equal. all: omega || auto.
-rewrite v_shift_negshift_comm. f_equal. assumption. omega.
+destruct h; simpl in *. auto.
+destruct novar. f_equal. auto.
+rewrite c_negshift_sub; try do 2 f_equal; aomega.
+rewrite v_shift_negshift_comm. f_equal. all: aomega.
 assert (S(S cut)=2+cut) as cc by omega; rewrite cc.
-apply v_no_var_shift. assumption. omega.
+apply v_no_var_shift; aomega.
 }
 Qed.
 
 
-Lemma v_sub_sub v v1 v2 i j :
+Fixpoint v_sub_sub v v1 v2 i j :
   v_no_var v j ->
-    v_sub v (i, v_sub v1 (j, v2))
-  = v_sub (v_sub v (i, v1)) (j, v2)
+  v_sub v (i, v_sub v1 (j, v2)) = v_sub (v_sub v (i, v1)) (j, v2)
 
 with c_sub_sub c v1 v2 i j :
   c_no_var c j ->
-    c_sub c (i, v_sub v1 (j, v2))
-  = c_sub (c_sub c (i, v1)) (j, v2)
+  c_sub c (i, v_sub v1 (j, v2)) = c_sub (c_sub c (i, v1)) (j, v2)
 
 with h_sub_sub h v1 v2 i j :
   h_no_var h j ->
-    h_sub h (i, v_sub v1 (j, v2))
-  = h_sub (h_sub h (i, v1)) (j, v2).
+  h_sub h (i, v_sub v1 (j, v2)) = h_sub (h_sub h (i, v1)) (j, v2).
+
 Proof.
+all: intros novar.
 {
-revert i j; induction v; intros i j novar; simpl.
-{ simpl. destruct (v=?i) eqn:cv. reflexivity.
-  simpl in *. assert (v=?j=false) by (apply Nat.eqb_neq; omega).
-  rewrite H. reflexivity. }
-all : simpl in novar; try destruct novar; f_equal; auto.
-all : rewrite v_shift_sub, c_sub_sub; omega || auto.
+destruct v; simpl in *; auto.
+{ destruct (n=?i) eqn:cn. auto. simpl. assert (n=?j=false) by
+  (apply Nat.eqb_neq; omega). rewrite H. auto. }
+all: try destruct novar; f_equal; auto.
+all: rewrite v_shift_sub, c_sub_sub; aomega.
 }{
-clear h_sub_sub.
-revert i j; induction c; intros i j novar; simpl.
-all : f_equal; simpl in novar; try destruct novar; auto.
-4: destruct H0; auto.
-all : rewrite v_shift_sub, c_sub_sub; omega || auto.
-all : destruct H0; auto.
+destruct c; simpl in *.
+all: f_equal; try destruct novar; try destruct H0; auto.
+all: rewrite v_shift_sub, c_sub_sub; aomega.
 }{
-clear v_sub_sub h_sub_sub.
-revert i j; induction h; intros i j novar; simpl.
-all : simpl in novar; f_equal; try destruct novar; auto.
-rewrite v_shift_sub, c_sub_sub; omega || auto.
+destruct h; simpl in *. auto.
+f_equal; try destruct novar; auto. rewrite v_shift_sub, c_sub_sub; aomega.
 }
 Qed.
 
@@ -728,37 +676,36 @@ Qed.
 Fixpoint v_under_var_subs v v' i j {struct v}:
   v_under_var v (S i) -> v_under_var v' i -> j <= i ->
   v_under_var (v_subs v j v') i
+
 with c_under_var_subs c v' i j {struct c}:
   c_under_var c (S i) -> v_under_var v' i -> j <= i ->
   c_under_var (c_subs c j v') i
+
 with h_under_var_subs h v' i j {struct h}:
   h_under_var h (S i) -> v_under_var v' i -> j <= i ->
   h_under_var (h_subs h j v') i.
+
 Proof.
-all: revert i j.
-+ intros. destruct v.
-  { unfold v_subs. simpl. simpl in H. destruct (v=?j) eqn:vj.
-    + rewrite v_negshift_shift, v_shift_0. auto. omega.
-    + simpl. destruct (j<=?v) eqn:cmp; simpl; apply Nat.eqb_neq in vj.
-      apply leb_complete in cmp. omega.
-      apply leb_complete_conv in cmp. omega. }
-  all: simpl in *; try inv H; try constructor.
-  all: try apply v_under_var_subs || apply h_under_var_subs; auto.
-  all: rewrite v_shift_comm; apply c_under_var_subs || omega; omega || auto.
-  all: apply v_under_var_shift; omega || assumption.
-+ intros. induction c; simpl in *; auto.
-  all: try constructor; try constructor; try inv H; auto.
-  all: try apply v_under_var_subs; eauto.
-  all: try destruct H3; eauto.
-  all: rewrite v_shift_comm; try apply c_under_var_subs; omega || auto.
-  all: try apply v_under_var_shift; omega || (try destruct H2; auto).
-  all: assert (S(S i) = 2+i) as same by omega; rewrite same.
-  all: apply v_under_var_shift; omega || assumption.
-+ intros. induction h; simpl in *; auto.
-  constructor; inv H; auto.
-  rewrite v_shift_comm; try apply c_under_var_subs; omega || auto.
-  assert (S(S i) = 2+i) by omega; rewrite H; apply v_under_var_shift.
-  assumption. omega.
+all: intros under under' cmp.
++ destruct v; simpl in *.
+  { unfold v_subs. simpl. destruct (n=?j) eqn:nj.
+  + rewrite v_negshift_shift, v_shift_0; aomega.
+  + simpl. destruct (j<=?n) eqn:cmpj; simpl; apply Nat.eqb_neq in nj.
+    apply leb_complete in cmpj. omega.
+    apply leb_complete_conv in cmpj. omega. }
+  all: try destruct under; try constructor; eauto.
+  all: rewrite v_shift_comm; eaomega; apply c_under_var_subs; aomega.
+  all: apply v_under_var_shift; aomega.
++ destruct c; simpl in *; eauto.
+  all: try destruct under; try destruct H0; try constructor; try constructor.
+  all: eauto; rewrite v_shift_comm; try apply c_under_var_subs; aomega.
+  all: assert (S(S i) = 2+i) as same by omega; try rewrite same.
+  all: apply v_under_var_shift; aomega.
++ destruct h; simpl in *; eauto.
+  destruct under. constructor. eauto.
+  rewrite v_shift_comm; try apply c_under_var_subs; aomega.
+  assert (S(S i) = 2+i) as same by omega; try rewrite same.
+  apply v_under_var_shift; aomega.
 Qed.
 
 
@@ -774,259 +721,165 @@ with h_no_var_subs h v' i j {struct h}:
   h_no_var h (1+i) -> v_no_var v' i -> j<=i ->
   h_no_var (h_subs h j v') i.
 Proof.
-all: revert i j.
-+ intros. destruct v.
-  { unfold v_subs. simpl. simpl in H.
-    destruct (v=?j) eqn:vj.
-    + rewrite v_negshift_shift, v_shift_0. auto. omega.
-    + simpl. destruct (j<=?v) eqn:jlv; simpl; apply Nat.eqb_neq in vj.
-      - apply leb_complete in jlv. omega.
-      - apply leb_complete_conv in jlv. omega. }
-  all: simpl in *; try inv H; try constructor.
-  all: try apply v_no_var_subs || apply h_no_var_subs; auto.
-  all: rewrite v_shift_comm; apply c_no_var_subs || omega; omega || auto.
-  all: apply v_no_var_shift; omega || assumption.
-+ intros. induction c; simpl in *; try constructor; try constructor.
-  all: try inv H; try inv H3; auto.
-  all: try apply v_no_var_subs; eauto.
-  all: rewrite v_shift_comm; try apply c_no_var_subs; omega || auto.
-  all: try apply v_no_var_shift; omega || auto.
-  all: assert (S(S i) = 2+i) as same by omega; rewrite same.
-  all: apply v_no_var_shift; omega || assumption.
-+ intros. induction h; simpl in *; auto. inv H; constructor; auto.
-  rewrite v_shift_comm; try apply c_no_var_subs; omega || auto.
-  assert (S(S i) = 2+i) by omega; rewrite H; apply v_no_var_shift.
-  assumption. omega.
+all: intros no_var no_var' cmp.
++ destruct v; simpl in *.
+  { unfold v_subs. simpl. destruct (n=?j) eqn:nj.
+  + rewrite v_negshift_shift, v_shift_0; aomega.
+  + simpl. destruct (j<=?n) eqn:cmpj; simpl; apply Nat.eqb_neq in nj.
+    apply leb_complete in cmpj. omega.
+    apply leb_complete_conv in cmpj. omega. }
+  all: try destruct no_var; try constructor; eauto.
+  all: rewrite v_shift_comm; eaomega; apply c_no_var_subs; aomega.
+  all: apply v_no_var_shift; aomega.
++ destruct c; simpl in *; eauto.
+  all: try destruct no_var; try destruct H0; try constructor; try constructor.
+  all: eauto; rewrite v_shift_comm; try apply c_no_var_subs; aomega.
+  all: assert (S(S i) = 2+i) as same by omega; try rewrite same.
+  all: apply v_no_var_shift; aomega.
++ destruct h; simpl in *; eauto.
+  destruct no_var. constructor. eauto.
+  rewrite v_shift_comm; try apply c_no_var_subs; aomega.
+  assert (S(S i) = 2+i) as same by omega; try rewrite same.
+  apply v_no_var_shift; aomega.
 Qed.
 
 
-Lemma v_shift_subs v v' i j (safe: j <= i): 
-    v_shift (v_subs v j v') 1 i
+(* ==================== Full Subs Distributivity ==================== *)
+
+Fixpoint v_shift_subs v v' i j (safe: j <= i): 
+    v_shift (v_subs v j v') 1 i 
   = (v_subs (v_shift v 1 (1+i)) j (v_shift v' 1 i))
 
 with c_shift_subs c v' i j (safe: j <= i): 
-    c_shift (c_subs c j v') 1 i
+    c_shift (c_subs c j v') 1 i 
   = (c_subs (c_shift c 1 (1+i)) j (v_shift v' 1 i))
 
 with h_shift_subs h v' i j (safe: j <= i): 
-    h_shift (h_subs h j v') 1 i
+    h_shift (h_subs h j v') 1 i 
   = (h_subs (h_shift h 1 (1+i)) j (v_shift v' 1 i)).
+
 Proof.
 {
-induction v; unfold v_subs; simpl.
-{
-clear v_shift_subs c_shift_subs h_shift_subs.
-rename v into n.
-destruct (n=?i) eqn:ni.
-apply Nat.eqb_eq in ni. subst.
-+ destruct (i=?j) eqn:eqij.
-  - apply Nat.eqb_eq in eqij. subst.
-    assert (1+j<=?j=false) by (apply leb_correct_conv; omega).
-    simpl in H. rewrite H. simpl.
-    assert (j=?j=true) by (apply Nat.eqb_eq; reflexivity).
-    rewrite H0. simpl. 
-    rewrite v_negshift_shift, v_negshift_shift, v_shift_shift, v_shift_shift. f_equal. omega. omega.
-  - assert (1+i<=?i=false) by (apply leb_correct_conv; omega).
-    simpl in H. rewrite H. simpl. apply leb_correct in safe as s.
-    rewrite s, eqij. simpl. rewrite s. assert (i<=?i-1=false).
-    { apply leb_correct_conv. apply Nat.eqb_neq in eqij. omega. } 
-    rewrite H0. reflexivity.
-+ destruct (n=?j) eqn:nj.
-  * apply Nat.eqb_eq in nj. subst.
-    assert (1+i<=?j=false) by (apply leb_correct_conv; omega).
-    simpl in H. rewrite H. simpl.
-    assert (j=?j=true) by (apply Nat.eqb_eq; omega).
-    rewrite H0, v_negshift_shift, v_negshift_shift, v_shift_0, v_shift_0.
-    reflexivity. omega. omega.
-  * destruct (i<=?n) eqn:iln; simpl.
-    - apply leb_complete in iln.
-      assert (j<=?n=true) by (apply leb_correct; omega). rewrite H. simpl.
-      assert (i<=?n-1=true).
-      { apply leb_correct. apply Nat.eqb_neq in ni. omega. }
-      rewrite H0. simpl. assert (1+i<=?n=true).
-      { apply leb_correct. apply Nat.eqb_neq in ni. omega. }
-      simpl in H1. rewrite H1. simpl. 
-      assert (1+n=?j=false) by (apply Nat.eqb_neq; omega).
-      simpl in H2. rewrite H2. simpl. assert (j<=? S n=true).
-      { apply leb_correct. omega. }
-      rewrite H3. do 2 f_equal. apply Nat.eqb_neq in ni. omega.
-    - apply leb_complete_conv in iln.
-      assert (1+i<=?n=false) by (apply leb_correct_conv; omega).
-      simpl in H. rewrite H. simpl. rewrite nj. simpl.
-      destruct (j<=?n) eqn:jln.
-      simpl. assert (i<=?n-1=false) by (apply leb_correct_conv; omega).
-      rewrite H0. reflexivity.
-      simpl. assert (i<=?n=false) by (apply leb_correct_conv; omega).
-      rewrite H0. reflexivity.
-}
-all: f_equal; auto.
-3: apply h_shift_subs; auto.
-all: clear v_shift_subs h_shift_subs; unfold c_subs in c_shift_subs.
-all: rewrite v_shift_comm; try omega.
-all: rewrite c_shift_subs; clear c_shift_subs; try omega.
-all: do 3 f_equal; rewrite (v_shift_comm 1 j); f_equal; try omega.
-all: rewrite (v_shift_comm 1 i); f_equal; omega.
+destruct v; unfold v_subs; simpl.
+{ destruct (n=?i) eqn:ni.
+  apply Nat.eqb_eq in ni. subst.
+  + destruct (i=?j) eqn:eqij.
+    - apply Nat.eqb_eq in eqij. subst.
+      assert (1+j<=?j=false) by (apply leb_correct_conv; omega).
+      simpl in H. rewrite H. simpl.
+      assert (j=?j=true) by (apply Nat.eqb_eq; auto).
+      rewrite H0. simpl. 
+      rewrite v_negshift_shift, v_negshift_shift.
+      rewrite v_shift_shift, v_shift_shift. f_equal. omega. omega.
+    - assert (1+i<=?i=false) by (apply leb_correct_conv; omega).
+      simpl in H. rewrite H. simpl. apply leb_correct in safe as s.
+      rewrite s, eqij. simpl. rewrite s. assert (i<=?i-1=false).
+      { apply leb_correct_conv. apply Nat.eqb_neq in eqij. omega. } 
+      rewrite H0. auto.
+  + destruct (n=?j) eqn:nj.
+    * apply Nat.eqb_eq in nj. subst.
+      assert (1+i<=?j=false) by (apply leb_correct_conv; omega).
+      simpl in H. rewrite H. simpl.
+      assert (j=?j=true) by (apply Nat.eqb_eq; omega).
+      rewrite H0, v_negshift_shift, v_negshift_shift, v_shift_0, v_shift_0.
+      all: aomega.
+    * destruct (i<=?n) eqn:iln; simpl.
+      - apply leb_complete in iln.
+        assert (j<=?n=true) by (apply leb_correct; omega). rewrite H. simpl.
+        assert (i<=?n-1=true).
+        { apply leb_correct. apply Nat.eqb_neq in ni. omega. }
+        rewrite H0. simpl. assert (1+i<=?n=true).
+        { apply leb_correct. apply Nat.eqb_neq in ni. omega. }
+        simpl in H1. rewrite H1. simpl. 
+        assert (1+n=?j=false) by (apply Nat.eqb_neq; omega).
+        simpl in H2. rewrite H2. simpl. assert (j<=? S n=true).
+        { apply leb_correct. omega. }
+        rewrite H3. do 2 f_equal. apply Nat.eqb_neq in ni. omega.
+      - apply leb_complete_conv in iln.
+        assert (1+i<=?n=false) by (apply leb_correct_conv; omega).
+        simpl in H. rewrite H. simpl. rewrite nj. simpl.
+        destruct (j<=?n) eqn:jln; simpl.
+        ++assert (i<=?n-1=false) by (apply leb_correct_conv; omega).
+          rewrite H0. auto.
+        ++assert (i<=?n=false) by (apply leb_correct_conv; omega).
+          rewrite H0. auto. }
+all: f_equal; eauto; unfold c_subs in *.
+all: rewrite v_shift_comm, (v_shift_comm 1 j), (v_shift_comm 1 i); aomega.
+all: rewrite c_shift_subs; aomega.
 }{
-destruct c; unfold c_subs; simpl; f_equal;
-try apply v_shift_subs; try assumption.
-all: clear v_shift_subs h_shift_subs; unfold c_subs in c_shift_subs.
-+ rewrite <-(v_shift_shift 1), (v_shift_comm 1 j).
-  rewrite (v_shift_comm 1 (1+j)), c_shift_subs. clear c_shift_subs. simpl.
-  do 2 f_equal. all: try omega. 
-  rewrite <-(v_shift_shift 1 1 0), (v_shift_comm 1 j), (v_shift_comm 1 (1+j)).
-  all: f_equal||omega||auto. 
-  rewrite (v_shift_comm 1 i), (v_shift_comm 1 (1+i)). do 2 f_equal. all: omega.
-+ rewrite v_shift_comm, c_shift_subs. clear c_shift_subs. do 3 f_equal.
-  rewrite (v_shift_comm 1 j), (v_shift_comm 1 i). do 2 f_equal. all: omega.
-+ rewrite v_shift_comm, c_shift_subs. clear c_shift_subs. do 3 f_equal.
-  rewrite (v_shift_comm 1 j), (v_shift_comm 1 i). do 2 f_equal. all: omega.
-+ rewrite v_shift_comm, c_shift_subs. do 3 f_equal.
-  rewrite (v_shift_comm 1 i). reflexivity. all: omega.
-+ rewrite <-(v_shift_shift 1), (v_shift_comm 1 j).
-  rewrite (v_shift_comm 1 (1+j)), c_shift_subs. clear c_shift_subs. simpl.
-  do 2 f_equal. all: try omega. 
-  rewrite <-(v_shift_shift 1 1 0), (v_shift_comm 1 j), (v_shift_comm 1 (1+j)).
-  all: f_equal||omega||auto. 
-  rewrite (v_shift_comm 1 i), (v_shift_comm 1 (1+i)). do 2 f_equal. all: omega.
-+ rewrite v_shift_comm, c_shift_subs. clear c_shift_subs. do 3 f_equal.
-  rewrite (v_shift_comm 1 j), (v_shift_comm 1 i). do 2 f_equal. all: omega.
-+ rewrite <-(v_shift_shift 1), (v_shift_comm 1 j).
-  rewrite (v_shift_comm 1 (1+j)), c_shift_subs. clear c_shift_subs. simpl.
-  do 2 f_equal. all: try omega. 
-  rewrite <-(v_shift_shift 1 1 0), (v_shift_comm 1 j), (v_shift_comm 1 (1+j)).
-  all: f_equal||omega||auto. 
-  rewrite (v_shift_comm 1 i), (v_shift_comm 1 (1+i)). do 2 f_equal. all: omega.
-+ rewrite v_shift_comm, c_shift_subs. clear c_shift_subs. do 3 f_equal.
-  rewrite (v_shift_comm 1 j), (v_shift_comm 1 i). do 2 f_equal. all: omega.
-+ rewrite v_shift_comm. rewrite c_shift_subs. clear c_shift_subs.
-  do 2 f_equal. rewrite (v_shift_comm). reflexivity. all: omega.
-+ rewrite v_shift_comm, c_shift_subs. clear c_shift_subs. do 3 f_equal.
-  rewrite (v_shift_comm 1 j), (v_shift_comm 1 i). do 2 f_equal. all: omega.
-+ rewrite v_shift_comm. rewrite c_shift_subs. clear c_shift_subs.
-  do 2 f_equal. rewrite (v_shift_comm). reflexivity. all: omega.
+destruct c; unfold c_subs in *; simpl; f_equal; eauto.
+all: rewrite v_shift_comm, c_shift_subs; aomega.
+all: do 3 f_equal; rewrite (v_shift_comm 1 j); aomega.
+all: f_equal; rewrite (v_shift_comm 1 i); aomega.
 }{
-destruct h; unfold h_subs; simpl. auto. f_equal.
-+ apply h_shift_subs. assumption.
-+ clear v_shift_subs h_shift_subs. unfold c_subs in c_shift_subs.
-  rewrite <-(v_shift_shift 1), (v_shift_comm 1 j).
-  rewrite (v_shift_comm 1 (1+j)), c_shift_subs. clear c_shift_subs. simpl.
-  do 2 f_equal. all: try omega. 
-  rewrite <-(v_shift_shift 1 1 0), (v_shift_comm 1 j), (v_shift_comm 1 (1+j)).
-  all: f_equal||omega||auto. 
-  rewrite (v_shift_comm 1 i), (v_shift_comm 1 (1+i)). do 2 f_equal. all: omega.
+destruct h; unfold h_subs; unfold c_subs in *; simpl; f_equal; eauto.
+rewrite v_shift_comm, c_shift_subs; aomega.
+rewrite (v_shift_comm 1 j), (v_shift_comm 1 i); aomega.
 }
 Qed.
 
 
 Lemma v_shift_subs_alt v v' i j (safe: i <= j): 
-    v_shift (v_subs v j v') 1 i
+    v_shift (v_subs v j v') 1 i 
   = (v_subs (v_shift v 1 i) (1+j) (v_shift v' 1 i))
 
 with c_shift_subs_alt c v' i j (safe: i <= j): 
-    c_shift (c_subs c j v') 1 i
+    c_shift (c_subs c j v') 1 i 
   = (c_subs (c_shift c 1 i) (1+j) (v_shift v' 1 i))
 
 with h_shift_subs_alt h v' i j (safe: i <= j): 
-    h_shift (h_subs h j v') 1 i
+    h_shift (h_subs h j v') 1 i 
   = (h_subs (h_shift h 1 i) (1+j) (v_shift v' 1 i)).
 Proof.
 {
 induction v; unfold v_subs; simpl.
-{
-clear v_shift_subs_alt c_shift_subs_alt h_shift_subs_alt.
-rename v into n.
-destruct (n=?i) eqn:ni.
-apply Nat.eqb_eq in ni. subst.
-+ destruct (i=?j) eqn:eqij.
-  - assert (i<=?i=true) by (apply leb_correct; omega).
-    rewrite H. simpl. rewrite eqij.
-    rewrite v_negshift_shift, v_negshift_shift, v_shift_0, v_shift_0.
-    reflexivity. omega. omega.
-  - assert (i<=?i=true) by (apply leb_correct; omega).
-    simpl in H. rewrite H. simpl. apply Nat.eqb_neq in eqij as ijeq. 
-    assert (j<=?i=false) by (apply leb_correct_conv; omega).
-    rewrite H0, eqij. simpl. rewrite H, H0. reflexivity.
-+ destruct (n=?j) eqn:nj.
-  * apply Nat.eqb_eq in nj. subst.
-    assert (i<=?j=true) by (apply leb_correct; omega).
-    simpl in H. rewrite H. simpl.
-    assert (j=?j=true) by (apply Nat.eqb_eq; omega).
-    rewrite H0, v_negshift_shift, v_negshift_shift, v_shift_0, v_shift_0.
-    reflexivity. omega. omega.
-  * destruct (i<=?n) eqn:iln; simpl.
-    - apply leb_complete in iln.
-      rewrite nj. simpl.
-      destruct (j<=?n) eqn:jn; simpl. apply Nat.eqb_neq in ni.
-      assert (i<=?n-1=true) by (apply leb_correct; omega).
-      rewrite H. f_equal. f_equal. omega.
-      apply leb_correct in iln. rewrite iln. reflexivity.
-    - apply leb_complete_conv in iln.
-      assert (j<=?n=false) by (apply leb_correct_conv; omega).
-      assert (i<=?n=false) by (apply leb_correct_conv; omega).
-      rewrite H. simpl. rewrite H0. simpl.
-      assert (n=?S j=false) by (apply Nat.eqb_neq; omega).
-      rewrite H1. simpl. 
-      assert (S j<=?n=false) by (apply leb_correct_conv; omega).
-      simpl in H2. rewrite H2. reflexivity.  
-      }
-all: f_equal; auto.
-3: apply h_shift_subs_alt; auto.
-all: clear v_shift_subs_alt h_shift_subs_alt; unfold c_subs in c_shift_subs_alt.
-all: rewrite v_shift_comm; try omega.
-all: rewrite c_shift_subs_alt; clear c_shift_subs_alt; try omega.
-all: do 3 f_equal; rewrite (v_shift_comm 1 (S j)); f_equal; try omega.
-all: rewrite (v_shift_comm 1 i); f_equal; omega.
+{ destruct (n=?i) eqn:ni.
+  apply Nat.eqb_eq in ni. subst.
+  + destruct (i=?j) eqn:eqij.
+    - assert (i<=?i=true) by (apply leb_correct; omega).
+      rewrite H. simpl. rewrite eqij.
+      rewrite v_negshift_shift, v_negshift_shift, v_shift_0, v_shift_0.
+      reflexivity. omega. omega.
+    - assert (i<=?i=true) by (apply leb_correct; omega).
+      simpl in H. rewrite H. simpl. apply Nat.eqb_neq in eqij as ijeq. 
+      assert (j<=?i=false) by (apply leb_correct_conv; omega).
+      rewrite H0, eqij. simpl. rewrite H, H0. reflexivity.
+  + destruct (n=?j) eqn:nj.
+    * apply Nat.eqb_eq in nj. subst.
+      assert (i<=?j=true) by (apply leb_correct; omega).
+      simpl in H. rewrite H. simpl.
+      assert (j=?j=true) by (apply Nat.eqb_eq; omega).
+      rewrite H0, v_negshift_shift, v_negshift_shift, v_shift_0, v_shift_0.
+      reflexivity. omega. omega.
+    * destruct (i<=?n) eqn:iln; simpl.
+      - apply leb_complete in iln.
+        rewrite nj. simpl.
+        destruct (j<=?n) eqn:jn; simpl. apply Nat.eqb_neq in ni.
+        assert (i<=?n-1=true) by (apply leb_correct; omega).
+        rewrite H. f_equal. f_equal. omega.
+        apply leb_correct in iln. rewrite iln. reflexivity.
+      - apply leb_complete_conv in iln.
+        assert (j<=?n=false) by (apply leb_correct_conv; omega).
+        assert (i<=?n=false) by (apply leb_correct_conv; omega).
+        rewrite H. simpl. rewrite H0. simpl.
+        assert (n=?S j=false) by (apply Nat.eqb_neq; omega).
+        rewrite H1. simpl. 
+        assert (S j<=?n=false) by (apply leb_correct_conv; omega).
+        simpl in H2. rewrite H2. reflexivity. }
+all: f_equal; eauto; unfold c_subs in *.
+all: rewrite v_shift_comm, (v_shift_comm 1 (S j)), (v_shift_comm 1 i); aomega.
+all: rewrite c_shift_subs_alt; aomega.
 }{
-destruct c; unfold c_subs; simpl; f_equal;
-try apply v_shift_subs_alt; try assumption.
-all: clear v_shift_subs_alt h_shift_subs_alt; unfold c_subs in c_shift_subs_alt.
-+ rewrite <-(v_shift_shift 1), (v_shift_comm 1 j).
-  rewrite (v_shift_comm 1 (1+j)), c_shift_subs_alt. clear c_shift_subs_alt. simpl. do 2 f_equal. all: try omega. f_equal. 
-  rewrite <-(v_shift_shift 1 1 0), (v_shift_comm 1 (S j)).
-  rewrite (v_shift_comm 1 (1+S j)). all: f_equal||omega||auto. 
-  rewrite v_shift_shift, v_shift_shift, (v_shift_comm _ i).
-  reflexivity. omega.
-+ rewrite v_shift_comm, c_shift_subs_alt. clear c_shift_subs_alt. do 3 f_equal.
-  rewrite (v_shift_comm 1 (S j)), (v_shift_comm 1 i). do 2 f_equal. all: omega.
-+ rewrite v_shift_comm, c_shift_subs_alt. clear c_shift_subs_alt. do 3 f_equal.
-  rewrite (v_shift_comm 1 (S j)), (v_shift_comm 1 i). do 2 f_equal. all: omega.
-+ rewrite <-v_shift_comm. rewrite c_shift_subs_alt. clear c_shift_subs_alt.
-  do 2 f_equal. rewrite <-v_shift_comm. reflexivity. all: omega.
-+ rewrite <-(v_shift_shift 1), (v_shift_comm 1 j).
-  rewrite (v_shift_comm 1 (1+j)), c_shift_subs_alt. clear c_shift_subs_alt. simpl. do 2 f_equal. all: try omega. f_equal. 
-  rewrite <-(v_shift_shift 1 1 0), (v_shift_comm 1 (S j)).
-  rewrite (v_shift_comm 1 (1+S j)). all: f_equal||omega||auto. 
-  rewrite v_shift_shift, v_shift_shift, (v_shift_comm _ i).
-  reflexivity. omega.
-+ rewrite v_shift_comm, c_shift_subs_alt. clear c_shift_subs_alt. do 3 f_equal.
-  rewrite (v_shift_comm 1 (S j)), (v_shift_comm 1 i). do 2 f_equal. all: omega.
-+ rewrite <-(v_shift_shift 1), (v_shift_comm 1 j).
-  rewrite (v_shift_comm 1 (1+j)), c_shift_subs_alt. clear c_shift_subs_alt. simpl. do 2 f_equal. all: try omega. f_equal. 
-  rewrite <-(v_shift_shift 1 1 0), (v_shift_comm 1 (S j)).
-  rewrite (v_shift_comm 1 (1+S j)). all: f_equal||omega||auto. 
-  rewrite v_shift_shift, v_shift_shift, (v_shift_comm _ i).
-  reflexivity. omega.
-+ rewrite v_shift_comm, c_shift_subs_alt. clear c_shift_subs_alt. do 3 f_equal.
-  rewrite (v_shift_comm 1 (S j)), (v_shift_comm 1 i). do 2 f_equal. all: omega.
-+ rewrite <-v_shift_comm. rewrite c_shift_subs_alt. clear c_shift_subs_alt.
-  do 2 f_equal. rewrite <-v_shift_comm. reflexivity. all: omega.
-+ rewrite v_shift_comm, c_shift_subs_alt. clear c_shift_subs_alt. do 3 f_equal.
-  rewrite (v_shift_comm 1 (S j)), (v_shift_comm 1 i). do 2 f_equal. all: omega.
-+ rewrite <-v_shift_comm. rewrite c_shift_subs_alt. clear c_shift_subs_alt.
-  do 2 f_equal. rewrite <-v_shift_comm. reflexivity. all: omega.
+destruct c; unfold c_subs in *; simpl; f_equal; eauto.
+all: rewrite v_shift_comm, c_shift_subs_alt; aomega.
+all: do 3 f_equal; rewrite (v_shift_comm 1 (S j)); aomega.
+all: f_equal; rewrite (v_shift_comm 1 i); aomega.
 }{
-destruct h; unfold h_subs; simpl. auto. f_equal.
-+ apply h_shift_subs_alt. assumption.
-+ clear v_shift_subs_alt h_shift_subs_alt. unfold c_subs in c_shift_subs_alt.
-  rewrite <-(v_shift_shift 1), (v_shift_comm 1 j).
-  rewrite (v_shift_comm 1 (1+j)), c_shift_subs_alt. clear c_shift_subs_alt. simpl. do 2 f_equal. all: try omega. f_equal. 
-  rewrite <-(v_shift_shift 1 1 0), (v_shift_comm 1 (S j)).
-  rewrite (v_shift_comm 1 (1+S j)). all: f_equal||omega||auto. 
-  rewrite v_shift_shift, v_shift_shift, (v_shift_comm _ i).
-  reflexivity. omega.
+destruct h; unfold h_subs; unfold c_subs in *; simpl; f_equal; eauto.
+rewrite v_shift_comm, c_shift_subs_alt; aomega.
+rewrite (v_shift_comm 1 (S j)), (v_shift_comm 1 i); aomega.
 }
 Qed.
-
 
 
 Lemma v_negshift_subs v v' i j (safe: j <= i): 
@@ -1043,11 +896,12 @@ with h_negshift_subs h v' i j (safe: j <= i):
   h_no_var h (1+i) -> v_no_var v' (i) ->
     h_negshift (h_subs h j v') 1 i
   = (h_subs (h_negshift h 1 (1+i)) j (v_negshift v' 1 i)).
+
 Proof.
 {
-intros nov nov'. destruct v; unfold v_subs; simpl.
+intros nov nov'. destruct v; unfold v_subs; simpl in *.
 { clear v_negshift_subs c_negshift_subs h_negshift_subs.
-  rename v into n. destruct (n=?j) eqn:nj.
+  destruct (n=?j) eqn:nj.
   apply Nat.eqb_eq in nj. subst.
   destruct (1+i <=? j) eqn:cmpij.
   3 : destruct (1+i <=? n) eqn:Sin. all: simpl.
@@ -1056,7 +910,7 @@ intros nov nov'. destruct v; unfold v_subs; simpl.
   + simpl in cmpij. rewrite cmpij. simpl.
     assert (j=?j=true) by (apply Nat.eqb_eq; omega).
     rewrite H, v_negshift_shift, v_shift_0, v_negshift_shift, v_shift_0.
-    reflexivity. omega. omega.
+    all: aomega.
   + apply leb_complete in Sin as sin. simpl in Sin.
     rewrite Sin. apply Nat.eqb_neq in nj.
     assert (j<=?n=true) by (apply leb_correct; omega). simpl in H.
@@ -1065,70 +919,41 @@ intros nov nov'. destruct v; unfold v_subs; simpl.
     { apply Nat.eqb_neq. simpl in nov. omega. }
     rewrite H1. simpl. assert (j<=?n-1=true).
     { apply leb_correct. omega. }
-    rewrite H2. reflexivity.
+    rewrite H2. auto.
   + apply leb_complete_conv in Sin as sin. simpl in Sin. rewrite Sin. simpl.  
     rewrite nj. apply Nat.eqb_neq in nj. simpl.
     destruct (j<=?n) eqn:jln.
     - simpl. assert (i<=?n-1=false).
       { apply leb_correct_conv. omega. }
-      rewrite H. reflexivity.
+      rewrite H. auto.
     - simpl. assert (i<=?n=false).
       { apply leb_correct_conv. apply leb_complete_conv in jln. omega. }
-      rewrite H. reflexivity. 
-}
-all: f_equal; simpl in nov.
-all: try apply v_negshift_subs; try omega || auto.
-all: try destruct nov; apply h_negshift_subs || auto; auto.
-all: unfold c_subs in c_negshift_subs; rewrite v_shift_comm; try omega.
-all: rewrite (c_negshift_subs c _ (S i) (S j)); clear c_negshift_subs.
-all: omega || (apply v_no_var_shift; omega || auto) || auto.
-all: rewrite v_shift_comm; do 4 f_equal; try rewrite v_shift_negshift_comm.
-all: omega || auto.
+      rewrite H. auto. }
+all: f_equal; try destruct nov; eauto.
+all: unfold c_subs in *; rewrite v_shift_comm; aomega.
+all: rewrite (c_negshift_subs c _ (S i) (S j)); aomega.
+all: try (apply v_no_var_shift; aomega).
+all: rewrite v_shift_comm; do 4 f_equal; aomega. 
+all: rewrite v_shift_negshift_comm; aomega.
 }{
-induction c; intros nov nov'; unfold c_subs; simpl in nov |-*; f_equal;
-try apply v_negshift_subs; try assumption.
-all: clear v_negshift_subs h_negshift_subs.
-all: try (destruct nov; assumption).
-all: unfold c_subs in c_negshift_subs; inv nov; try destruct H0.
-+ rewrite <-(v_shift_shift 1), (v_shift_comm 1 j); try omega.
-  rewrite (v_shift_comm 1 (1+j)), c_negshift_subs; omega || auto. do 3 f_equal.
-  rewrite <-(v_shift_shift 1 1 0), (v_shift_comm 1 j), (v_shift_comm 1 (1+j));
-  try omega || f_equal; rewrite v_shift_shift, v_shift_shift.
-  rewrite v_shift_negshift_comm; omega || auto.
-  apply v_no_var_shift. apply v_no_var_shift. all: omega || auto.
-+ rewrite v_shift_comm, c_negshift_subs. do 3 f_equal.
-  rewrite <-v_shift_negshift_comm, <-v_shift_comm. all: omega || auto.
-  apply v_no_var_shift. auto. omega.
-+ rewrite v_shift_comm, c_negshift_subs. do 3 f_equal.
-  rewrite <-v_shift_negshift_comm, <-v_shift_comm. all: omega || auto.
-  apply v_no_var_shift. auto. omega.
-+ apply c_negshift_subs; omega || auto.
-+ rewrite v_shift_comm, c_negshift_subs. do 3 f_equal.
-  rewrite v_shift_comm. f_equal. rewrite v_shift_negshift_comm. 
-  all: omega || auto. rewrite <-(v_shift_shift 1 1). 
-  apply v_no_var_shift. apply v_no_var_shift. all: omega || auto.
-+ rewrite v_shift_comm, c_negshift_subs. do 3 f_equal.
-  rewrite <-v_shift_negshift_comm, <-v_shift_comm. all: omega || auto.
-  apply v_no_var_shift. auto. omega.
-+ rewrite v_shift_comm, c_negshift_subs. do 3 f_equal.
-  rewrite v_shift_comm. f_equal. rewrite v_shift_negshift_comm. 
-  all: omega || auto. rewrite <-(v_shift_shift 1 1). 
-  apply v_no_var_shift. apply v_no_var_shift. all: omega || auto.
-+ rewrite v_shift_comm, c_negshift_subs. do 3 f_equal.
-  rewrite <-v_shift_negshift_comm, <-v_shift_comm. all: omega || auto.
-  apply v_no_var_shift. auto. omega.
-+ apply c_negshift_subs; omega || auto.
-+ rewrite v_shift_comm, c_negshift_subs. do 3 f_equal.
-  rewrite <-v_shift_negshift_comm, <-v_shift_comm. all: omega || auto.
-  apply v_no_var_shift. auto. omega.
-+ apply c_negshift_subs; omega || auto.
+intros nov nov'; destruct c; unfold c_subs in *; simpl in *.
+all: try destruct nov; try destruct H0; f_equal; eauto.
+all: rewrite v_shift_comm; aomega; simpl.
+all: assert (S(S i)=2+i) as ssi by (omega).
+all: try rewrite (c_negshift_subs _ _ (S i) (S j))
+  || rewrite (c_negshift_subs _ _ (S(S i)) (S(S j))); aomega.
+all: try rewrite ssi; try (apply v_no_var_shift; aomega).
+all: rewrite v_shift_comm; do 4 f_equal; aomega. 
+all: rewrite v_shift_negshift_comm; aomega.
 }{
-destruct h; unfold h_subs; intros nov nov'; simpl. auto. inv nov. f_equal.
-+ apply h_negshift_subs; auto.
-+ unfold c_subs in c_negshift_subs. clear v_negshift_subs h_negshift_subs.
-  rewrite <-(v_shift_shift 1), (v_shift_comm 1 j).
-  rewrite (v_shift_comm 1 (1+j)), c_negshift_subs. clear c_negshift_subs. rewrite <-(v_shift_shift 1 1 0), (v_shift_comm 1 j), (v_shift_comm 1 (1+j)). do 4 f_equal. rewrite v_shift_shift, v_shift_shift, v_shift_negshift_comm.
-  all: try (apply v_no_var_shift; omega||apply v_no_var_shift); omega||auto.
+intros nov nov'; destruct h; unfold c_subs in *; unfold h_subs in *; simpl in *.
+all: try destruct nov; f_equal; eauto.
+rewrite v_shift_comm; aomega; simpl.
+assert (S(S i)=2+i) as ssi by (omega).
+rewrite (c_negshift_subs _ _ (S(S i)) (S(S j))); aomega.
+2: rewrite ssi; (apply v_no_var_shift; aomega).
+rewrite v_shift_comm; do 4 f_equal; aomega. 
+rewrite v_shift_negshift_comm; aomega.
 }
 Qed.
 
@@ -1148,18 +973,19 @@ with h_negshift_subs_alt h v' i j (safe: j >= i):
   h_no_var h i -> v_no_var v' (i) ->
     h_negshift (h_subs h (1+j) v') 1 i
   = (h_subs (h_negshift h 1 i) j (v_negshift v' 1 i)).
+
 Proof.
 {
 intros nov nov'. destruct v; unfold v_subs; simpl.
 { clear v_negshift_subs_alt c_negshift_subs_alt h_negshift_subs_alt.
-  rename v into n. destruct (n=?S j) eqn:nSj.
+  destruct (n=?S j) eqn:nSj.
   apply Nat.eqb_eq in nSj. subst.
   2 : destruct (i <=? n) eqn:cmpin. all: simpl.
   + assert(i<=?S j=true) by (apply leb_correct; omega).
     rewrite H. simpl.
     assert(j-0=?j=true) by (apply Nat.eqb_eq; omega).
     rewrite H0, v_negshift_shift, v_shift_0, v_negshift_shift, v_shift_0.
-    auto. omega. omega.
+    all: aomega.
   + apply leb_complete in cmpin as ccmpin.
     apply Nat.eqb_neq in nSj as nnSj. simpl in nov.
     assert (n-1=?j=false) by (apply Nat.eqb_neq; omega).
@@ -1169,10 +995,10 @@ intros nov nov'. destruct v; unfold v_subs; simpl.
       assert (S j<=?n=true) by (apply leb_correct; omega).
       simpl in H0. rewrite H0. simpl.
       assert (i<=?n-1=true) by (apply leb_correct; omega).
-      rewrite H1. reflexivity.
+      rewrite H1. auto.
     - apply leb_complete_conv in jnm1.
       assert (1+j<=?n=false) by (apply leb_correct_conv; omega).
-      simpl in H0. rewrite H0. simpl. rewrite cmpin. reflexivity.
+      simpl in H0. rewrite H0. simpl. rewrite cmpin. auto.
   + apply leb_complete_conv in cmpin as ccmpin.
     apply Nat.eqb_neq in nSj as nnSj. simpl in nov.
     assert (n=?j=false) by (apply Nat.eqb_neq; omega).
@@ -1180,67 +1006,37 @@ intros nov nov'. destruct v; unfold v_subs; simpl.
     assert (j<=?n=false) by (apply leb_correct_conv; omega).
     rewrite H0.
     assert (1+j<=?n=false) by (apply leb_correct_conv; omega).
-    simpl in H1. rewrite H1. simpl. rewrite cmpin. reflexivity.
-}
-all: f_equal; simpl in nov.
-all: try apply v_negshift_subs_alt; try omega || auto.
-all: try destruct nov; apply h_negshift_subs_alt || auto; auto.
-all: unfold c_subs in c_negshift_subs_alt; rewrite v_shift_comm; try omega.
-all: rewrite (c_negshift_subs_alt c _ (S i) (S j)); clear c_negshift_subs_alt.
-all: omega || (apply v_no_var_shift; omega || auto) || auto.
-all: rewrite v_shift_comm; do 4 f_equal; try rewrite v_shift_negshift_comm.
-all: omega || auto.
+    simpl in H1. rewrite H1. simpl. rewrite cmpin. auto. }
+all: f_equal; try destruct nov; eauto.
+all: unfold c_subs in *; rewrite v_shift_comm; aomega.
+all: rewrite (c_negshift_subs_alt c _ (S i) (S j)); aomega.
+all: try (apply v_no_var_shift; aomega).
+all: rewrite v_shift_comm; do 4 f_equal; aomega. 
+all: rewrite v_shift_negshift_comm; aomega.
 }{
-destruct c; intros nov nov'; unfold c_subs; simpl in nov |-*; f_equal;
-try apply v_negshift_subs_alt; try assumption.
-all: clear v_negshift_subs_alt h_negshift_subs_alt.
-all: try (destruct nov; assumption).
-all: unfold c_subs in c_negshift_subs_alt; inv nov; try destruct H0.
-+ rewrite <-(v_shift_shift 1), (v_shift_comm 1 j); try omega.
-  rewrite (v_shift_comm 1 (1+j)), (v_shift_comm 1 (1+(1+j))).
-  rewrite (c_negshift_subs_alt _ _). all: omega || auto. do 4 f_equal.
-  rewrite (v_shift_shift), v_shift_negshift_comm. all: omega || auto.
-  apply v_no_var_shift. apply v_no_var_shift. all: omega || auto.
-+ rewrite v_shift_comm, c_negshift_subs_alt. do 3 f_equal.
-  rewrite <-v_shift_negshift_comm, <-v_shift_comm. all: omega || auto.
-  apply v_no_var_shift. auto. omega.
-+ rewrite v_shift_comm, c_negshift_subs_alt. do 3 f_equal.
-  rewrite <-v_shift_negshift_comm, <-v_shift_comm. all: omega || auto.
-  apply v_no_var_shift. auto. omega.
-+ apply c_negshift_subs_alt; omega || auto.
-+ rewrite v_shift_comm, c_negshift_subs_alt. do 3 f_equal.
-  rewrite v_shift_comm. f_equal. rewrite v_shift_negshift_comm. 
-  all: omega || auto. rewrite <-(v_shift_shift 1 1). 
-  apply v_no_var_shift. apply v_no_var_shift. all: omega || auto.
-+ rewrite v_shift_comm, c_negshift_subs_alt. do 3 f_equal.
-  rewrite <-v_shift_negshift_comm, <-v_shift_comm. all: omega || auto.
-  apply v_no_var_shift. auto. omega.
-+ rewrite v_shift_comm, c_negshift_subs_alt. do 3 f_equal.
-  rewrite v_shift_comm. f_equal. rewrite v_shift_negshift_comm. 
-  all: omega || auto. rewrite <-(v_shift_shift 1 1). 
-  apply v_no_var_shift. apply v_no_var_shift. all: omega || auto.
-+ rewrite v_shift_comm, c_negshift_subs_alt. do 3 f_equal.
-  rewrite <-v_shift_negshift_comm, <-v_shift_comm. all: omega || auto.
-  apply v_no_var_shift. auto. omega.
-+ apply c_negshift_subs_alt; omega || auto.
-+ rewrite v_shift_comm, c_negshift_subs_alt. do 3 f_equal.
-  rewrite <-v_shift_negshift_comm, <-v_shift_comm. all: omega || auto.
-  apply v_no_var_shift. auto. omega.
-+ apply c_negshift_subs_alt; omega || auto.
+intros nov nov'; destruct c; unfold c_subs in *; simpl in *.
+all: try destruct nov; try destruct H0; f_equal; eauto.
+all: rewrite v_shift_comm; aomega; simpl.
+all: assert (S(S i)=2+i) as ssi by (omega).
+all: try rewrite (c_negshift_subs_alt _ _ (S i) (S j))
+  || rewrite (c_negshift_subs_alt _ _ (S(S i)) (S(S j))); aomega.
+all: try rewrite ssi; try (apply v_no_var_shift; aomega).
+all: rewrite v_shift_comm; do 4 f_equal; aomega. 
+all: rewrite v_shift_negshift_comm; aomega.
 }{
-destruct h; unfold h_subs; intros nov nov'; simpl. auto. inv nov. f_equal.
-+ apply h_negshift_subs_alt; auto.
-+ unfold c_subs in c_negshift_subs_alt. clear v_negshift_subs_alt h_negshift_subs_alt.
-  rewrite <-(v_shift_shift 1), (v_shift_comm 1 j); try omega.
-  rewrite (v_shift_comm 1 (1+j)), (v_shift_comm 1 (1+(1+j))).
-  rewrite (c_negshift_subs_alt _ _). all: omega || auto. do 4 f_equal.
-  rewrite (v_shift_shift), v_shift_negshift_comm. all: omega || auto.
-  apply v_no_var_shift. apply v_no_var_shift. all: omega || auto.
+intros nov nov'; destruct h; unfold c_subs in *; unfold h_subs in *; simpl in *.
+all: try destruct nov; f_equal; eauto.
+rewrite v_shift_comm; aomega; simpl.
+assert (S(S i)=2+i) as ssi by (omega).
+rewrite (c_negshift_subs_alt _ _ (S(S i)) (S(S j))); aomega.
+2: rewrite ssi; (apply v_no_var_shift; aomega).
+rewrite v_shift_comm; do 4 f_equal; aomega. 
+rewrite v_shift_negshift_comm; aomega.
 }
 Qed.
 
 
-Lemma v_sub_subs v i j vi vj:
+Fixpoint v_sub_subs v i j vi vj:
   j >= i ->
     v_sub (v_subs v i vi) (j, vj)
   = (v_subs (v_sub v (1+j, v_shift vj 1 i)) i (v_sub vi (j, vj)))
@@ -1256,64 +1052,56 @@ with h_sub_subs h i j vi vj:
   = (h_subs (h_sub h (1+j, v_shift vj 1 i)) i (v_sub vi (j, vj))).
 Proof.
 {
-intros cmp. induction v; unfold v_subs; simpl.
-{
-clear v_sub_subs c_sub_subs h_sub_subs.
-rename v into n.
-destruct (n=?i) eqn:ni.
-apply Nat.eqb_eq in ni. subst.
-+ assert (i=?S j=false) by (apply Nat.eqb_neq; omega). rewrite H.
-  destruct (i=?j) eqn:eqij.
-  - apply Nat.eqb_eq in eqij. simpl.
-    assert (i=?i=true) by (apply Nat.eqb_eq; omega). rewrite H0.
-    rewrite v_negshift_shift, v_negshift_shift, v_shift_0, v_shift_0.
-    reflexivity. omega. omega.
-  - simpl. assert (i=?i=true) by (apply Nat.eqb_eq; omega).
-    rewrite H0, v_negshift_shift, v_negshift_shift.
-    rewrite v_shift_0, v_shift_0. reflexivity. all: omega.
-+ destruct (n=?S j) eqn:nsj.
-  - apply Nat.eqb_eq in nsj. subst. simpl.
-    assert (i<=?S j=true) by (apply leb_correct; omega).
-    rewrite H. simpl. assert (j-0=?j=true) by (apply Nat.eqb_eq; omega).
-    rewrite H0, v_sub_no_var, v_negshift_shift, v_shift_0.
-    reflexivity. omega. apply v_shift_makes_no_var.
-  - simpl. rewrite ni. simpl. destruct (i<=?n) eqn:cmpin.
-    * simpl. assert (n-1=?j=false).
-      { apply leb_complete in cmpin. apply Nat.eqb_neq.
-        apply Nat.eqb_neq in nsj. apply Nat.eqb_neq in ni. omega. }
-      rewrite H. reflexivity.
-    * simpl. assert (n=?j=false).
-      { apply Nat.eqb_neq. apply leb_complete_conv in cmpin. omega. }
-      rewrite H. reflexivity.
-}
-all: f_equal; auto.
-3: apply h_sub_subs; auto.
-all: clear v_sub_subs h_sub_subs; unfold c_subs in c_sub_subs.
-all: rewrite v_shift_comm, c_sub_subs; clear c_sub_subs; try omega.
-all: do 2 f_equal; try rewrite <-v_shift_sub; try omega.
-all: try rewrite <-v_shift_comm; try omega; f_equal.
+intros cmp. destruct v; unfold v_subs; simpl in *.
+{ destruct (n=?i) eqn:ni.
+  apply Nat.eqb_eq in ni. subst.
+  + assert (i=?S j=false) by (apply Nat.eqb_neq; omega). rewrite H.
+    destruct (i=?j) eqn:eqij.
+    - apply Nat.eqb_eq in eqij. simpl.
+      assert (i=?i=true) by (apply Nat.eqb_eq; omega). rewrite H0.
+      rewrite v_negshift_shift, v_negshift_shift, v_shift_0, v_shift_0.
+      reflexivity. omega. omega.
+    - simpl. assert (i=?i=true) by (apply Nat.eqb_eq; omega).
+      rewrite H0, v_negshift_shift, v_negshift_shift.
+      rewrite v_shift_0, v_shift_0. reflexivity. all: omega.
+  + destruct (n=?S j) eqn:nsj.
+    - apply Nat.eqb_eq in nsj. subst. simpl.
+      assert (i<=?S j=true) by (apply leb_correct; omega).
+      rewrite H. simpl. assert (j-0=?j=true) by (apply Nat.eqb_eq; omega).
+      rewrite H0, v_sub_no_var_same, v_negshift_shift, v_shift_0.
+      reflexivity. omega. apply v_shift_makes_no_var.
+    - simpl. rewrite ni. simpl. destruct (i<=?n) eqn:cmpin.
+      * simpl. assert (n-1=?j=false).
+        { apply leb_complete in cmpin. apply Nat.eqb_neq.
+          apply Nat.eqb_neq in nsj. apply Nat.eqb_neq in ni. omega. }
+        rewrite H. reflexivity.
+      * simpl. assert (n=?j=false).
+        { apply Nat.eqb_neq. apply leb_complete_conv in cmpin. omega. }
+        rewrite H. reflexivity. }
+all: f_equal; eauto.
+all: unfold c_subs in *; rewrite v_shift_comm, c_sub_subs; aomega.
+all: do 2 f_equal; try rewrite <-v_shift_sub; aomega.
+all: try rewrite <-v_shift_comm; aomega.
 }{
-intros cmp. induction c; unfold c_subs; simpl; f_equal; auto.
-all: try apply v_sub_subs; try assumption.
-all: clear v_sub_subs h_sub_subs; unfold c_subs in c_sub_subs.
-all: try rewrite v_shift_comm, c_sub_subs; try omega.
-all: do 2 f_equal; try rewrite <-v_shift_sub; try omega.
-all: try rewrite <-v_shift_comm; try omega; f_equal.
-all: rewrite (v_shift_comm _ i); f_equal; try omega.
-all: rewrite v_shift_sub; f_equal; omega.
+intros cmp. destruct c; unfold c_subs in *; simpl in *; f_equal; eauto.
+all: rewrite v_shift_comm, c_sub_subs; aomega.
+all: do 2 f_equal; try rewrite <-v_shift_sub; aomega.
+all: try rewrite <-v_shift_comm; aomega.
+all: assert (S(S i)=2+i) as ssi by (omega); rewrite ssi.
+all: try rewrite <-v_shift_comm; aomega.
+all: rewrite v_shift_comm; aomega; do 2 f_equal; rewrite v_shift_sub; aomega.
 }{
-intros cmp. induction h; unfold h_subs; simpl; f_equal; auto.
-unfold c_subs in c_sub_subs. rewrite v_shift_comm, c_sub_subs; try omega.
-do 2 f_equal; try rewrite <-v_shift_sub; try omega.
-all: try rewrite <-v_shift_comm; try omega; f_equal.
-rewrite (v_shift_comm _ i); f_equal; try omega.
-rewrite v_shift_comm. f_equal. rewrite v_shift_sub. f_equal.
-all: omega.
+intros cmp. destruct h; unfold h_subs in *; unfold c_subs in *;
+simpl in *; f_equal; eauto.
+assert (S(S i)=2+i) as ssi by (omega); rewrite ssi.
+rewrite v_shift_comm, c_sub_subs; aomega.
+do 2 f_equal. rewrite <-v_shift_comm; aomega.
+rewrite v_shift_comm; aomega. do 2 f_equal; rewrite v_shift_sub; aomega.
 }
 Qed.
 
 
-Lemma v_sub_subs_alt v i j vi vj:
+Fixpoint v_sub_subs_alt v i j vi vj:
   j < i ->
     v_sub (v_subs v i vi) (j, vj)
   = (v_subs (v_sub v (j, v_shift vj 1 i)) i (v_sub vi (j, vj)))
@@ -1327,56 +1115,49 @@ with h_sub_subs_alt h i j vi vj:
   j < i ->
     h_sub (h_subs h i vi) (j, vj)
   = (h_subs (h_sub h (j, v_shift vj 1 i)) i (v_sub vi (j, vj))).
+
 Proof.
 {
-intros cmp. induction v; unfold v_subs; simpl.
-{
-clear v_sub_subs_alt c_sub_subs_alt h_sub_subs_alt.
-rename v into n.
-destruct (n=?i) eqn:ni.
-apply Nat.eqb_eq in ni. subst.
-+ assert (i=?j=false) by (apply Nat.eqb_neq; omega).
-  rewrite H. simpl.
-  assert (i=?i=true) by (apply Nat.eqb_eq; omega).
-  rewrite H0, v_negshift_shift, v_negshift_shift.
-  rewrite v_shift_0, v_shift_0. reflexivity. all: omega.
-+ destruct (n=?j) eqn:nj.
-  - apply Nat.eqb_eq in nj. subst. simpl.
-    assert (i<=?j=false) by (apply leb_correct_conv; omega).
+intros cmp. destruct v; unfold v_subs; simpl.
+{ destruct (n=?i) eqn:ni.
+  apply Nat.eqb_eq in ni. subst.
+  + assert (i=?j=false) by (apply Nat.eqb_neq; omega).
     rewrite H. simpl.
-    assert (j=?j=true) by (apply Nat.eqb_eq; omega).
-    rewrite H0, v_sub_no_var, v_negshift_shift, v_shift_0.
-    reflexivity. omega. apply v_shift_makes_no_var.
-  - simpl. rewrite ni. simpl. destruct (i<=?n) eqn:cmpin.
-    * simpl. assert (n-1=?j=false).
-      { apply leb_complete in cmpin. apply Nat.eqb_neq.
-        apply Nat.eqb_neq in nj. apply Nat.eqb_neq in ni. omega. }
-      rewrite H. reflexivity.
-    * simpl. rewrite nj. reflexivity. 
-}
-all: f_equal; auto.
-3: apply h_sub_subs_alt; auto.
-all: clear v_sub_subs_alt h_sub_subs_alt; unfold c_subs in c_sub_subs_alt.
-all: rewrite v_shift_comm, c_sub_subs_alt; clear c_sub_subs_alt; try omega.
-all: do 2 f_equal; try rewrite <-v_shift_sub; try omega.
-all: try rewrite <-v_shift_comm; try omega; f_equal.
+    assert (i=?i=true) by (apply Nat.eqb_eq; omega).
+    rewrite H0, v_negshift_shift, v_negshift_shift.
+    rewrite v_shift_0, v_shift_0. all: aomega.
+  + destruct (n=?j) eqn:nj.
+    - apply Nat.eqb_eq in nj. subst. simpl.
+      assert (i<=?j=false) by (apply leb_correct_conv; omega).
+      rewrite H. simpl.
+      assert (j=?j=true) by (apply Nat.eqb_eq; omega).
+      rewrite H0, v_sub_no_var_same, v_negshift_shift, v_shift_0; aomega.
+      apply v_shift_makes_no_var.
+    - simpl. rewrite ni. simpl. destruct (i<=?n) eqn:cmpin.
+      * simpl. assert (n-1=?j=false).
+        { apply leb_complete in cmpin. apply Nat.eqb_neq.
+          apply Nat.eqb_neq in nj. apply Nat.eqb_neq in ni. omega. }
+        rewrite H. auto.
+      * simpl. rewrite nj. auto. }
+all: f_equal; eauto.
+all: unfold c_subs in *; rewrite v_shift_comm, c_sub_subs_alt; aomega.
+all: do 2 f_equal; try rewrite <-v_shift_sub; aomega.
+all: try rewrite <-v_shift_comm; aomega.
 }{
-intros cmp. induction c; unfold c_subs; simpl; f_equal; auto.
-all: try apply v_sub_subs_alt; try assumption.
-all: clear v_sub_subs_alt h_sub_subs_alt; unfold c_subs in c_sub_subs_alt.
-all: try rewrite v_shift_comm, c_sub_subs_alt; try omega.
-all: do 2 f_equal; try rewrite <-v_shift_sub; try omega.
-all: try rewrite <-v_shift_comm; try omega; f_equal.
-all: rewrite (v_shift_comm _ i); f_equal; try omega.
-all: rewrite v_shift_sub; f_equal; omega.
+intros cmp. destruct c; unfold c_subs in *; simpl in *; f_equal; eauto.
+all: rewrite v_shift_comm, c_sub_subs_alt; aomega.
+all: do 2 f_equal; try rewrite <-v_shift_sub; aomega.
+all: try rewrite <-v_shift_comm; aomega.
+all: assert (S(S i)=2+i) as ssi by (omega); rewrite ssi.
+all: try rewrite <-v_shift_comm; aomega.
+all: rewrite v_shift_comm; aomega; do 2 f_equal; rewrite v_shift_sub; aomega.
 }{
-intros cmp. induction h; unfold h_subs; simpl; f_equal; auto.
-unfold c_subs in c_sub_subs_alt. rewrite v_shift_comm, c_sub_subs_alt; try omega.
-do 2 f_equal; try rewrite <-v_shift_sub; try omega.
-all: try rewrite <-v_shift_comm; try omega; f_equal.
-rewrite (v_shift_comm _ i); f_equal; try omega.
-rewrite v_shift_comm. f_equal. rewrite v_shift_sub. f_equal.
-all: omega.
+intros cmp. destruct h; unfold h_subs in *; unfold c_subs in *;
+simpl in *; f_equal; eauto.
+assert (S(S i)=2+i) as ssi by (omega); rewrite ssi.
+rewrite v_shift_comm, c_sub_subs_alt; aomega.
+do 2 f_equal. rewrite <-v_shift_comm; aomega.
+rewrite v_shift_comm; aomega. do 2 f_equal; rewrite v_shift_sub; aomega.
 }
 Qed.
 
@@ -1395,28 +1176,24 @@ with h_subs_subs h i j vi vj:
   j >= i ->
     h_subs (h_subs h i vi) j vj
   = (h_subs (h_subs h (1+j) (v_shift vj 1 i)) i (v_subs vi j vj)).
+
 Proof.
+all: intros cmp.
 {
-intro cmp.
-assert (v_subs v i vi=v_negshift(v_sub v (i, v_shift vi 1 i)) 1 i). reflexivity. unfold v_subs. rewrite <-H.
-rewrite v_sub_subs, v_negshift_subs, v_shift_comm.
-all: try reflexivity || omega.
-all: apply v_sub_makes_no_var. rewrite v_shift_comm. 2: omega. 
-all: apply v_shift_makes_no_var. 
+specialize v_sub_subs as vss. specialize v_negshift_subs as vns.
+unfold v_subs in *. rewrite vss, vns, v_shift_comm; aomega.
+all: apply v_sub_makes_no_var. rewrite v_shift_comm; aomega.
+all: apply v_shift_makes_no_var.
 }{
-intro cmp.
-assert (c_subs c i vi=c_negshift(c_sub c (i, v_shift vi 1 i)) 1 i). reflexivity. unfold c_subs. rewrite <-H.
-rewrite c_sub_subs, c_negshift_subs, v_shift_comm.
-all: try reflexivity || omega.
-apply c_sub_makes_no_var. rewrite v_shift_comm. 2: omega. 
-2: apply v_sub_makes_no_var. all: apply v_shift_makes_no_var. 
+specialize c_sub_subs as css. specialize c_negshift_subs as cns.
+unfold c_subs in *. rewrite css, cns, v_shift_comm; aomega.
+all: apply c_sub_makes_no_var || apply v_sub_makes_no_var.
+rewrite v_shift_comm; aomega. all: apply v_shift_makes_no_var.
 }{
-intro cmp.
-assert (h_subs h i vi=h_negshift(h_sub h (i, v_shift vi 1 i)) 1 i). reflexivity. unfold h_subs. rewrite <-H.
-rewrite h_sub_subs, h_negshift_subs, v_shift_comm.
-all: try reflexivity || omega.
-apply h_sub_makes_no_var. rewrite v_shift_comm. 2: omega. 
-2: apply v_sub_makes_no_var. all: apply v_shift_makes_no_var. 
+specialize h_sub_subs as hss. specialize h_negshift_subs as hns.
+unfold h_subs in *. rewrite hss, hns, v_shift_comm; aomega.
+all: apply h_sub_makes_no_var || apply v_sub_makes_no_var.
+rewrite v_shift_comm; aomega. all: apply v_shift_makes_no_var.
 }
 Qed.
 
@@ -1436,33 +1213,22 @@ with h_subs_subs_alt h i j vi vj:
     h_subs (h_subs h (1+i) vi) j vj
   = (h_subs (h_subs h j (v_shift vj 1 i)) i (v_subs vi j vj)).
 Proof.
+all: intros cmp.
 {
-intro cmp.
-assert (v_subs v (1+i) vi
-  =v_negshift(v_sub v (1+i, v_shift vi 1 (1+i))) 1 (1+i)). 
-reflexivity. unfold v_subs. rewrite <-H.
-rewrite v_sub_subs_alt, v_negshift_subs_alt, <-v_shift_comm.
-all: try reflexivity || omega.
-all: apply v_sub_makes_no_var. rewrite <-v_shift_comm. 2: omega. 
-all: apply v_shift_makes_no_var. 
+specialize v_sub_subs_alt as vss. specialize v_negshift_subs_alt as vns.
+unfold v_subs in *. rewrite vss, vns, <-v_shift_comm; aomega.
+all: apply v_sub_makes_no_var. rewrite <-v_shift_comm; aomega.
+all: apply v_shift_makes_no_var.
 }{
-intro cmp.
-assert (c_subs c (1+i) vi
-  =c_negshift(c_sub c ((1+i), v_shift vi 1 (1+i))) 1 (1+i)). 
-reflexivity. unfold c_subs. rewrite <-H.
-rewrite c_sub_subs_alt, c_negshift_subs_alt, <-v_shift_comm.
-all: try reflexivity || omega.
-apply c_sub_makes_no_var. rewrite <-v_shift_comm. 2: omega. 
-2: apply v_sub_makes_no_var. all: apply v_shift_makes_no_var. 
+specialize c_sub_subs_alt as css. specialize c_negshift_subs_alt as cns.
+unfold c_subs in *. rewrite css, cns, <-v_shift_comm; aomega.
+all: apply c_sub_makes_no_var || apply v_sub_makes_no_var.
+rewrite <-v_shift_comm; aomega. all: apply v_shift_makes_no_var.
 }{
-intro cmp.
-assert (h_subs h (1+i) vi
-  =h_negshift(h_sub h ((1+i), v_shift vi 1 (1+i))) 1 (1+i)). 
-reflexivity. unfold h_subs. rewrite <-H.
-rewrite h_sub_subs_alt, h_negshift_subs_alt, <-v_shift_comm.
-all: try reflexivity || omega.
-apply h_sub_makes_no_var. rewrite <-v_shift_comm. 2: omega. 
-2: apply v_sub_makes_no_var. all: apply v_shift_makes_no_var. 
+specialize h_sub_subs_alt as hss. specialize h_negshift_subs_alt as hns.
+unfold h_subs in *. rewrite hss, hns, <-v_shift_comm; aomega.
+all: apply h_sub_makes_no_var || apply v_sub_makes_no_var.
+rewrite <-v_shift_comm; aomega. all: apply v_shift_makes_no_var.
 }
 Qed.
 
@@ -1475,7 +1241,7 @@ revert i j. induction I; intros; simpl; f_equal; auto.
 Qed.
 
 Lemma get_inst_val_shift I n d c :
-  get_inst_val (inst_shift I d c) n 
+    get_inst_val (inst_shift I d c) n 
   = f_opt (get_inst_val I n) (fun v => Some (v_shift v d c)).
 Proof.
 revert n d c. induction I; intros; simpl in *. auto. 
@@ -1484,7 +1250,7 @@ Qed.
 
 
 Lemma get_inst_val_negshift I n d c :
-  get_inst_val (inst_negshift I d c) n 
+    get_inst_val (inst_negshift I d c) n 
   = f_opt (get_inst_val I n) (fun v => Some (v_negshift v d c)).
 Proof.
 revert n d c. induction I; intros; simpl in *. auto. 
@@ -1493,7 +1259,7 @@ Qed.
 
 
 Lemma get_inst_val_sub I n i v:
-  get_inst_val (inst_sub I (i, v)) n 
+    get_inst_val (inst_sub I (i, v)) n 
   = f_opt (get_inst_val I n) (fun v' => Some (v_sub v' (i, v))).
 Proof.
 revert n. induction I; intros; simpl in *. auto. 
@@ -1510,19 +1276,19 @@ with h_shift_inst I h d cut:
 Proof.
 {
 destruct v; simpl; eauto.
-{ rewrite get_inst_val_shift. destruct (get_inst_val I v); simpl; auto. }
+{ rewrite get_inst_val_shift. destruct (get_inst_val I n); simpl; auto. }
 all: f_equal; eauto.
-all: rewrite inst_shift_comm; simpl; omega || eauto.
+all: rewrite inst_shift_comm; simpl; eaomega.
 all: apply c_shift_inst; auto.
 }{
 destruct c; simpl; eauto.
 all: f_equal; eauto.
-all: rewrite inst_shift_comm; simpl; omega || eauto.
+all: rewrite inst_shift_comm; simpl; eaomega.
 all: apply c_shift_inst; auto.
 }{
 destruct h; simpl; eauto.
 all: f_equal; eauto.
-all: rewrite inst_shift_comm; simpl; omega || eauto.
+all: rewrite inst_shift_comm; simpl; eaomega.
 all: apply c_shift_inst; auto.
 }
 Qed.
@@ -1531,36 +1297,39 @@ Qed.
 Fixpoint v_negshift_inst I v cut:
   inst_no_var I cut ->
   v_negshift (v_inst v I) 1 cut = v_inst v (inst_negshift I 1 cut)
+
 with c_negshift_inst I c cut:
   inst_no_var I cut ->
   c_negshift (c_inst c I) 1 cut = c_inst c (inst_negshift I 1 cut)
+
 with h_negshift_inst I h cut:
   inst_no_var I cut ->
   h_negshift (h_inst h I) 1 cut = h_inst h (inst_negshift I 1 cut).
+
 Proof.
 {
 intros. destruct v; simpl; eauto.
-{ rewrite get_inst_val_negshift. destruct (get_inst_val I v); simpl; auto. }
+{ rewrite get_inst_val_negshift. destruct (get_inst_val I n); simpl; auto. }
 all: f_equal; eauto.
-all: rewrite inst_shift_negshift_comm; simpl; omega || eauto.
+all: rewrite inst_shift_negshift_comm; simpl; eaomega.
 all: apply c_negshift_inst; simpl; constructor.
-all: omega || apply inst_no_var_shift; omega || eauto.
+all: try apply inst_no_var_shift; eaomega.
 }{
 assert (S(S cut) = 2+cut) as same by omega.
 intros. destruct c; simpl; eauto.
 all: f_equal; eauto.
-all: rewrite inst_shift_negshift_comm; simpl; omega || eauto.
+all: rewrite inst_shift_negshift_comm; simpl; eaomega.
 all: apply c_negshift_inst; try omega.
 all: simpl; constructor; try constructor; try rewrite same.
-all: try apply inst_no_var_shift; omega || eauto.
+all: try apply inst_no_var_shift; eaomega.
 }{
 assert (S(S cut) = 2+cut) as same by omega.
 intros. destruct h; simpl; eauto.
 all: f_equal; eauto.
-all: rewrite inst_shift_negshift_comm; simpl; omega || eauto.
+all: rewrite inst_shift_negshift_comm; simpl; eaomega.
 all: apply c_negshift_inst; try omega.
 all: simpl; constructor; try constructor; try rewrite same.
-all: try apply inst_no_var_shift; omega || eauto.
+all: try apply inst_no_var_shift; eaomega.
 }
 Qed.
 
@@ -1574,19 +1343,19 @@ with h_sub_inst I h i vs:
 Proof.
 {
 destruct v; simpl; eauto.
-{ rewrite get_inst_val_sub. destruct (get_inst_val I v); simpl; auto. }
+{ rewrite get_inst_val_sub. destruct (get_inst_val I n); simpl; auto. }
 all: f_equal; eauto.
-all: rewrite inst_shift_sub; simpl; omega || eauto.
+all: rewrite inst_shift_sub; simpl; eaomega.
 all: apply c_sub_inst.
 }{
 destruct c; simpl; eauto.
 all: f_equal; eauto.
-all: rewrite inst_shift_sub; simpl; omega || eauto.
+all: rewrite inst_shift_sub; simpl; eaomega.
 all: apply c_sub_inst.
 }{
 destruct h; simpl; eauto.
 all: f_equal; eauto.
-all: rewrite inst_shift_sub; simpl; omega || eauto.
+all: rewrite inst_shift_sub; simpl; eaomega.
 all: apply c_sub_inst.
 }
 Qed.
@@ -1595,8 +1364,7 @@ Qed.
 Lemma inst_subs_unfold I i v_s:
   inst_negshift (inst_sub I (i, v_shift v_s 1 i)) 1 i = inst_subs I i v_s.
 Proof.
-revert i. induction I; intros; simpl. auto.
-rewrite IHI. f_equal.
+revert i. induction I; intros; simpl. auto. rewrite IHI. auto.
 Qed.
 
 
@@ -1609,31 +1377,29 @@ with h_subs_inst I h vs i:
 Proof.
 {
 unfold v_subs. 
-rewrite v_sub_inst, v_negshift_inst, inst_subs_unfold. all: auto.
+rewrite v_sub_inst, v_negshift_inst, inst_subs_unfold; auto.
 apply inst_sub_makes_no_var. apply v_shift_makes_no_var.
 }{
 unfold c_subs. 
-rewrite c_sub_inst, c_negshift_inst, inst_subs_unfold. all: auto.
+rewrite c_sub_inst, c_negshift_inst, inst_subs_unfold; auto.
 apply inst_sub_makes_no_var. apply v_shift_makes_no_var.
 }{
 unfold h_subs. 
-rewrite h_sub_inst, h_negshift_inst, inst_subs_unfold. all: auto.
+rewrite h_sub_inst, h_negshift_inst, inst_subs_unfold; auto.
 apply inst_sub_makes_no_var. apply v_shift_makes_no_var.
 }
 Qed.
 
 
 Fixpoint inst_shift_insert I n v i {struct I}:
-  inst_shift (inst_insert I n v) i 0 
+    inst_shift (inst_insert I n v) i 0 
   = inst_insert (inst_shift I i 0) n (v_shift v i 0).
 Proof.
-destruct I; simpl.
-+ destruct (n=?0) eqn:n0; simpl; auto.
-+ destruct (n=?0); simpl; auto. f_equal. auto.
+destruct I; simpl; destruct (n=?0); simpl; auto. f_equal. auto.
 Qed.
 
 
-Lemma instU_inst_insert I i vs v:
+Lemma inst_insert_extend I i vs v:
   InstU (inst_insert I i vs) v = inst_insert (InstU I v) (S i) vs.
 Proof.
   simpl. do 2 f_equal. omega.
@@ -1641,39 +1407,45 @@ Qed.
 
 
 Fixpoint v_inst_no_var_same I vs i v:
-  v_no_var v i -> v_under_var v (1+inst_len I) -> i <= inst_len I ->
+  v_no_var v i -> v_under_var v (1+inst_len I) ->
+  i <= inst_len I ->
   v_inst v (inst_insert I i vs) = v_inst (v_negshift v 1 i) I
+
 with c_inst_no_var_same I vs i c:
-  c_no_var c i -> c_under_var c (1+inst_len I) -> i <= inst_len I ->
+  c_no_var c i -> c_under_var c (1+inst_len I) -> 
+  i <= inst_len I ->
   c_inst c (inst_insert I i vs) = c_inst (c_negshift c 1 i) I
+
 with h_inst_no_var_same I vs i h:
-  h_no_var h i -> h_under_var h (1+inst_len I) -> i <= inst_len I ->
+  h_no_var h i -> h_under_var h (1+inst_len I) ->
+  i <= inst_len I ->
   h_inst h (inst_insert I i vs) = h_inst (h_negshift h 1 i) I.
+
 Proof.
 {
 intros safe under ilen. destruct v; simpl; auto.
-{ rename v into dbi. destruct (i<=?dbi) eqn:cmp.
+{ destruct (i<=?n) eqn:cmp.
   + apply leb_complete in cmp. simpl in *.
-    destruct dbi. omega. 
+    destruct n. omega. 
     rewrite inst_insert_above. simpl.
-    assert (dbi-0=dbi) by omega. rewrite H. all: omega || auto.
+    assert (n-0=n) by omega. rewrite H. all: eaomega.
   + apply leb_complete_conv in cmp. simpl in *.
-    rewrite inst_insert_under. simpl. all: omega || auto. }
+    rewrite inst_insert_under. simpl. all: eaomega. }
 all: f_equal; simpl in *; try destruct safe; try destruct under; eauto.
-all: rewrite inst_shift_insert, instU_inst_insert.
-all: apply c_inst_no_var_same; simpl; omega || auto.
-all: rewrite inst_len_shift; omega || auto.
+all: rewrite inst_shift_insert, inst_insert_extend.
+all: apply c_inst_no_var_same; simpl; eaomega.
+all: rewrite inst_len_shift; eaomega.
 }{
 intros safe under ilen. destruct c; simpl.
 all: f_equal; simpl in *; try destruct safe; try destruct under; eauto.
-all: try rewrite inst_shift_insert, instU_inst_insert.
-all: try rewrite instU_inst_insert; try apply c_inst_no_var_same; simpl; auto.
-all: try rewrite inst_len_shift; omega || auto.
+all: try rewrite inst_shift_insert, inst_insert_extend.
+all: try rewrite inst_insert_extend; try apply c_inst_no_var_same; simpl; auto.
+all: try rewrite inst_len_shift; eaomega.
 all: try destruct H0; auto; destruct H2; auto.
 }{
 intros safe under ilen. destruct h; simpl. auto.
 f_equal; simpl in *; destruct safe; destruct under. auto.
-rewrite inst_shift_insert, instU_inst_insert, instU_inst_insert.
+rewrite inst_shift_insert, inst_insert_extend, inst_insert_extend.
 apply c_inst_no_var_same; auto; simpl; rewrite inst_len_shift. auto. omega.
 }
 Qed.
